SoftwareFoundations/ProgrammingLanguageFoundations/Equiv.lean
@@ -24,51 +24,53 @@ namespace SoftwareFoundations.ProgrammingLanguageFoundations.Equiv
   @[reducible] def _root_.SoftwareFoundations.LogicalFoundations.Imp.Command.equiv (c₁ c₂: Command): Prop := ∀ s₁ s₂: State, CommandEval c₁ s₁ s₂ ↔ CommandEval c₂ s₁ s₂
   @[reducible] def _root_.SoftwareFoundations.LogicalFoundations.Imp.Command.refines (c₁ c₂: Command): Prop := ∀ s₁ s₂: State, CommandEval c₁ s₁ s₂ → CommandEval c₂ s₁ s₂
 
-  namespace Term
-    example: (Arith.minus "X" "X").equiv (Arith.num 0) :=
-      fun s =>
-        calc (Arith.minus "X" "X").eval s
-          _ = (s "X") - (s "X")    := rfl
-          _ = 0                    := Nat.sub_self (s "X")
-          _ = (Arith.num 0).eval s := rfl
+  infix:50 "≈" => Arith.equiv
+  infix:50 "≈" => Logic.equiv
+  infix:50 "≈" => Command.equiv
 
-    example: (Logic.eq (.minus "X" "X") 0).equiv .true :=
+  namespace Term
+    example: [Arith| X - X] ≈ [Arith| 0] :=
       fun s =>
-        calc (Logic.eq (.minus "X" "X") 0).eval s
+        calc [Arith| X - X].eval s
+          _ = (s "X") - (s "X") := rfl
+          _ = 0                 := Nat.sub_self (s "X")
+          _ = [Arith| 0].eval s := rfl
+
+    example: [Logic| (X - X) = 0] ≈ [Logic| tru] :=
+      fun s =>
+        calc [Logic| (X - X) = 0].eval s
           _ = BEq.beq ((s "X") - (s "X")) 0 := rfl
           _ = BEq.beq 0 0                   := congrFun (congrArg BEq.beq (Nat.sub_self (s "X"))) 0
-          _ = .true                         := rfl
+          _ = [Logic| tru].eval s           := rfl
   end Term
 
   namespace Tactic
-    example: (Arith.minus "X" "X").equiv (Arith.num 0) := by
+    example: [Arith| X - X] ≈ [Arith| 0] := by
       unfold Arith.equiv
       intro s
       simp
 
-    example: (Logic.eq (.minus "X" "X") 0).equiv .true := by
+    example: [Logic| (X - X) = 0] ≈ [Logic| tru] := by
       unfold Logic.equiv
       intro s
       simp
-      unfold Arith.eval
-      rfl
   end Tactic
 
   namespace Blended
-    example: (Arith.minus "X" "X").equiv (Arith.num 0) :=
+    example: [Arith| X - X] ≈ [Arith| 0] :=
       fun s =>
-        calc (Arith.minus "X" "X").eval s
-          _ = (s "X") - (s "X")    := by rfl
-          _ = 0                    := by rw [Nat.sub_self]
-          _ = (Arith.num 0).eval s := by rfl
+        calc [Arith| X - X].eval s
+          _ = (s "X") - (s "X") := by rfl
+          _ = 0                 := by rw [Nat.sub_self]
+          _ = [Arith| 0].eval s := by rfl
 
 
-    example: (Logic.eq (.minus "X" "X") 0).equiv .true :=
+    example: [Logic| (X - X) = 0] ≈ [Logic| tru] :=
       fun s =>
-        calc (Logic.eq (.minus "X" "X") 0).eval s
+        calc [Logic| (X - X) = 0].eval s
           _ = BEq.beq ((s "X") - (s "X")) 0 := by rfl
           _ = BEq.beq 0 0                   := by rw [Nat.sub_self]
-          _ = .true                         := by rfl
+          _ = [Logic| tru].eval s           := by rfl
   end Blended
 
   /-
@@ -79,11 +81,11 @@ namespace SoftwareFoundations.ProgrammingLanguageFoundations.Equiv
     False.elim (by simp_all)
 
   namespace Term
-    theorem Command.skip_left {c: Command}: (Command.seq .skip c).equiv c
-      | s₁, s₂ =>
-        have mp: CommandEval (Command.seq .skip c) s₁ s₂ → CommandEval c s₁ s₂
+    theorem Command.skip_left {c: Command}: [Imp| skip; <[ c ]>] ≈ c
+      | _, _ =>
+        have mp
           | .seq _ _ _ (.skip _) h₂ => h₂
-        have mpr: CommandEval c s₁ s₂ → CommandEval (Command.seq .skip c) s₁ s₂
+        have mpr
           | .skip _                   => .seq _ _ _ (.skip _) (.skip _)
           | .assign _ h               => .seq _ _ _ (.skip _) (.assign _ h)
           | .seq _ _ _ h₁ h₂          => .seq _ _ _ (.skip _) (.seq _ _ _ h₁ h₂)
@@ -93,11 +95,11 @@ namespace SoftwareFoundations.ProgrammingLanguageFoundations.Equiv
           | .whileFalse _ h₁          => .seq _ _ _ (.skip _) (.whileFalse _ h₁)
         ⟨mp, mpr⟩
 
-    theorem Command.skip_right {c: Command}: (Command.seq c .skip).equiv c
-      | s₁, s₂ =>
-        have mp: CommandEval (Command.seq c .skip) s₁ s₂ → CommandEval c s₁ s₂
+    theorem Command.skip_right {c: Command}: [Imp| <[ c ]>; skip] ≈ c
+      | _, _ =>
+        have mp
           | .seq _ _ _ h₁ (.skip _) => h₁
-        have mpr: CommandEval c s₁ s₂ → CommandEval (Command.seq c .skip) s₁ s₂
+        have mpr
           | .skip _                   => .seq _ _ _ (.skip _) (.skip _)
           | .assign _ h               => .seq _ _ _ (.assign _ h) (.skip _)
           | .seq _ _ _ h₁ h₂          => .seq _ _ _ (.seq _ _ _ h₁ h₂) (.skip _)
@@ -107,12 +109,12 @@ namespace SoftwareFoundations.ProgrammingLanguageFoundations.Equiv
           | .whileFalse _ h₁          => .seq _ _ _ (.whileFalse _ h₁) (.skip _)
         ⟨mp, mpr⟩
 
-    example {t f: Command}: (Command.if .true t f).equiv t
-      | s₁, s₂ =>
-        have mp: CommandEval (.if .true t f) s₁ s₂ → CommandEval t s₁ s₂
+    example {t f: Command}: [Imp| ite (tru) { <[t]> } else { <[f]> }] ≈ t
+      | _, _ =>
+        have mp
           | .ifTrue _ _ _ h₂ => h₂
           | .ifFalse _ _ h₁ _ => Logic.true.trueFalse rfl h₁
-        have mpr: CommandEval t s₁ s₂ → CommandEval (.if .true t f) s₁ s₂
+        have mpr
           | .skip _                   => .ifTrue _ _ rfl (.skip _)
           | .assign _ h               => .ifTrue _ _ rfl (.assign _ h)
           | .seq _ _ _ h₁ h₂          => .ifTrue _ _ rfl (.seq _ _ _ h₁ h₂)
@@ -122,111 +124,111 @@ namespace SoftwareFoundations.ProgrammingLanguageFoundations.Equiv
           | .whileFalse _ h           => .ifTrue _ _ rfl (.whileFalse _ h)
         ⟨mp, mpr⟩
 
-    theorem Command.if_true {b: Logic} {c₁ c₂: Command} (h: b.equiv .true): (Command.if b c₁ c₂).equiv c₁
-      | s₁, s₂ =>
-        have tru: b.eval s₁ = Logic.true.eval s₁ := h _
-        have mp: CommandEval (.if b c₁ c₂) s₁ s₂ → CommandEval c₁ s₁ s₂
+    theorem Command.if_true {b: Logic} {c₁ c₂: Command} (h: b ≈ .true): [Imp| ite (<[expr:b]>) { <[ c₁ ]> } else { <[ c₂ ]> }] ≈ c₁
+      | _, _ =>
+        have truu: b.eval _ = Logic.true.eval _ := h _
+        have mp
           | .ifTrue _ _ _ h₂ => h₂
-          | .ifFalse _ _ h₁ _ => b.trueFalse tru h₁
-        have mpr: CommandEval c₁ s₁ s₂ → CommandEval (.if b c₁ c₂) s₁ s₂
-          | .skip _                   => .ifTrue _ _ tru (.skip _)
-          | .assign _ h₁              => .ifTrue _ _ tru (.assign _ h₁)
-          | .seq _ _ _ h₁ h₂          => .ifTrue _ _ tru (.seq _ _ _ h₁ h₂)
-          | .ifTrue _ _ h₁ h₂         => .ifTrue _ _ tru (.ifTrue _ _ h₁ h₂)
-          | .ifFalse _ _ h₁ h₂        => .ifTrue _ _ tru (.ifFalse _ _ h₁ h₂)
-          | .whileTrue _ _ _ h₁ h₂ h₃ => .ifTrue _ _ tru (.whileTrue _ _ _ h₁ h₂ h₃)
-          | .whileFalse _ h₁          => .ifTrue _ _ tru (.whileFalse _ h₁)
+          | .ifFalse _ _ h₁ _ => b.trueFalse truu h₁
+        have mpr
+          | .skip _                   => .ifTrue _ _ truu (.skip _)
+          | .assign _ h₁              => .ifTrue _ _ truu (.assign _ h₁)
+          | .seq _ _ _ h₁ h₂          => .ifTrue _ _ truu (.seq _ _ _ h₁ h₂)
+          | .ifTrue _ _ h₁ h₂         => .ifTrue _ _ truu (.ifTrue _ _ h₁ h₂)
+          | .ifFalse _ _ h₁ h₂        => .ifTrue _ _ truu (.ifFalse _ _ h₁ h₂)
+          | .whileTrue _ _ _ h₁ h₂ h₃ => .ifTrue _ _ truu (.whileTrue _ _ _ h₁ h₂ h₃)
+          | .whileFalse _ h₁          => .ifTrue _ _ truu (.whileFalse _ h₁)
         ⟨mp, mpr⟩
 
-    theorem Command.if_false {b: Logic} {c₁ c₂: Command} (h: b.equiv .false): (Command.if b c₁ c₂).equiv c₂
-      | s₁, s₂ =>
-        have fls: b.eval s₁ = Logic.false.eval s₁ := h _
-        have mp: CommandEval (.if b c₁ c₂) s₁ s₂ → CommandEval c₂ s₁ s₂
-          | .ifTrue _ _ h₁ _ => b.trueFalse h₁ fls
+    theorem Command.if_false {b: Logic} {c₁ c₂: Command} (h: b ≈ .false): [Imp| ite (<[expr:b]>) { <[ c₁ ]> } else { <[ c₂ ]> }] ≈ c₂
+      | _, _ =>
+        have falz: b.eval _ = Logic.false.eval _ := h _
+        have mp
+          | .ifTrue _ _ h₁ _ => b.trueFalse h₁ falz
           | .ifFalse _ _ _ h₂ => h₂
-        have mpr: CommandEval c₂ s₁ s₂ → CommandEval (.if b c₁ c₂) s₁ s₂
-          | .skip _                   => .ifFalse _ _ fls (.skip _)
-          | .assign _ h₁              => .ifFalse _ _ fls (.assign _ h₁)
-          | .seq _ _ _ h₁ h₂          => .ifFalse _ _ fls (.seq _ _ _ h₁ h₂)
-          | .ifTrue _ _ h₁ h₂         => .ifFalse _ _ fls (.ifTrue _ _ h₁ h₂)
-          | .ifFalse _ _ h₁ h₂        => .ifFalse _ _ fls (.ifFalse _ _ h₁ h₂)
-          | .whileTrue _ _ _ h₁ h₂ h₃ => .ifFalse _ _ fls (.whileTrue _ _ _ h₁ h₂ h₃)
-          | .whileFalse _ h₁          => .ifFalse _ _ fls (.whileFalse _ h₁)
+        have mpr
+          | .skip _                   => .ifFalse _ _ falz (.skip _)
+          | .assign _ h₁              => .ifFalse _ _ falz (.assign _ h₁)
+          | .seq _ _ _ h₁ h₂          => .ifFalse _ _ falz (.seq _ _ _ h₁ h₂)
+          | .ifTrue _ _ h₁ h₂         => .ifFalse _ _ falz (.ifTrue _ _ h₁ h₂)
+          | .ifFalse _ _ h₁ h₂        => .ifFalse _ _ falz (.ifFalse _ _ h₁ h₂)
+          | .whileTrue _ _ _ h₁ h₂ h₃ => .ifFalse _ _ falz (.whileTrue _ _ _ h₁ h₂ h₃)
+          | .whileFalse _ h₁          => .ifFalse _ _ falz (.whileFalse _ h₁)
         ⟨mp, mpr⟩
 
-    theorem Command.if_swap {b: Logic} {c₁ c₂: Command}: (Command.if b c₁ c₂).equiv (Command.if (.not b) c₂ c₁)
-      | s₁, s₂ =>
-        have mp: CommandEval (.if b c₁ c₂) s₁ s₂ → CommandEval (.if (.not b) c₂ c₁) s₁ s₂ := sorry
-        have mpr: CommandEval (.if (.not b) c₂ c₁) s₁ s₂ → CommandEval (.if b c₁ c₂) s₁ s₂ := sorry
+    theorem Command.if_swap {b: Logic} {c₁ c₂: Command}: [Imp| ite (<[expr:b]>) { <[ c₁ ]> } else { <[ c₂ ]> }] ≈ [Imp| ite ( ! <[expr:b]> ) { <[ c₂ ]> } else { <[ c₁ ]> }]
+      | _, _ =>
+        have mp := sorry
+        have mpr := sorry
         ⟨mp, mpr⟩
 
-    theorem Command.while_false {c: Logic} {b: Command} (h: c.equiv .false): (Command.while c b).equiv Command.skip
-      | s₁, s₂ =>
-        have fls: c.eval s₁ = Logic.false.eval s₁ := h _
-        have mp: CommandEval (.while c b) s₁ s₂ → CommandEval .skip s₁ s₂
-          | .whileTrue _ _ _ h₁ _ _=> c.trueFalse h₁ fls
+    theorem Command.while_false {c: Logic} {b: Command} (h: c ≈ .false): [Imp| while (<[expr:c]>) { <[b]> }] ≈ [Imp| skip]
+      | _, _ =>
+        have falz: c.eval _ = Logic.false.eval _ := h _
+        have mp
+          | .whileTrue _ _ _ h₁ _ _=> c.trueFalse h₁ falz
           | .whileFalse _ _ => .skip _
-        have mpr: CommandEval .skip s₁ s₂ → CommandEval (.while c b) s₁ s₂
-          | .skip _ => .whileFalse _ fls
+        have mpr
+          | .skip _ => .whileFalse _ falz
         ⟨mp, mpr⟩
 
-    theorem Command.while_true {c: Logic} {b: Command} (h: c.equiv .true): (Command.while c b).equiv (Command.while .true Command.skip)
-      | s₁, s₂ =>
-        have tru: c.eval s₁ = Logic.true.eval s₁ := h _
+    theorem Command.while_true {c: Logic} {b: Command} (h: c ≈ .true): [Imp| while (<[expr:c]>) { <[b]> }] ≈ [Imp| while (tru) { skip }]
+      | _, _ =>
+        have truu: c.eval _ = Logic.true.eval _ := h _
         have hh: Logic.true.equiv .true
           | _ => rfl
-        have mp: CommandEval (.while c b) s₁ s₂ → CommandEval (.while .true .skip) s₁ s₂
+        have mp
           | .whileTrue _ _ _ h₁ h₂ h₃ => absurd (CommandEval.whileTrue _ _ _ h₁ h₂ h₃) (nonterm h)
-          | .whileFalse _ h₁ => c.trueFalse tru h₁
-        have mpr: CommandEval (.while .true .skip) s₁ s₂ → CommandEval (.while c b) s₁ s₂
+          | .whileFalse _ h₁ => c.trueFalse truu h₁
+        have mpr
           | .whileTrue _ _ _ h₁ h₂ h₃ => absurd (CommandEval.whileTrue _ _ _ h₁ h₂ h₃) (nonterm hh)
           | .whileFalse _ h₁ => Logic.true.trueFalse rfl h₁
         ⟨mp, mpr⟩
       where
-        nonterm {c: Logic} {b: Command} {s₁ s₂: State} (h: c.equiv .true): ¬(CommandEval (.while c b) s₁ s₂)
+        nonterm {c: Logic} {b: Command} {s₁ s₂: State} (h: c ≈ .true): ¬(s₁ =[[Imp| while (<[expr:c]>) { <[ b ]> }]]=> s₂)
           | .whileTrue s₁ s₂ s₃ h₁ h₂ h₃ =>
             sorry
           | .whileFalse _ h₁ => c.trueFalse (h _) h₁
 
-    theorem Command.loop_unrolling {c: Logic} {b: Command}: (Command.while c b).equiv (Command.if c (Command.seq b (Command.while c b)) .skip)
-      | s₁, s₂ =>
-        have mp: CommandEval (.while c b) s₁ s₂ → CommandEval (.if c (.seq b (.while c b)) .skip) s₁ s₂
+    theorem Command.loop_unrolling {c: Logic} {b: Command}: [Imp| while (<[expr:c]>) { <[b]> }] ≈ [Imp| ite (<[expr:c]>) { <[b]>; while (<[expr:c]>) { <[b]> }} else { skip }]
+      | _, _ =>
+        have mp
           | .whileTrue _ _ _ h₁ h₂ h₃ => .ifTrue _ _ h₁ (.seq _ _ _ h₂ h₃)
           | .whileFalse _ h₁ => .ifFalse _ _ h₁ (.skip _)
-        have mpr: CommandEval (.if c (.seq b (.while c b)) .skip) s₁ s₂ → CommandEval (.while c b) s₁ s₂
+        have mpr
           | .ifTrue _ _ h₁ (.seq _ _ _ h₂ h₃) => .whileTrue _ _ _ h₁ h₂ h₃
           | .ifFalse _ _ h₁ (.skip _) => .whileFalse _ h₁
         ⟨mp, mpr⟩
 
-    theorem Command.seq_assoc {c₁ c₂ c₃: Command}: (Command.seq (Command.seq c₁ c₂) c₃).equiv (Command.seq c₁ (Command.seq c₂ c₃))
-      | s₁, s₂ =>
-        have mp: CommandEval (.seq (.seq c₁ c₂) c₃) s₁ s₂ → CommandEval (.seq c₁ (.seq c₂ c₃)) s₁ s₂
+    theorem Command.seq_assoc {c₁ c₂ c₃: Command}: [Imp| (<[c₁]>; <[c₂]>); <[c₃]>] ≈ [Imp| <[c₁]>; (<[c₂]>; <[c₃]>)]
+      | _, _ =>
+        have mp
           | .seq _ _ _ (.seq _ _ _ h₁ h₂) h₃ => .seq _ _ _ h₁ (.seq _ _ _ h₂ h₃)
-        have mpr: CommandEval (.seq c₁ (.seq c₂ c₃)) s₁ s₂ → CommandEval (.seq (.seq c₁ c₂) c₃) s₁ s₂
+        have mpr
           | .seq _ _ _ h₁ (.seq _ _ _ h₂ h₃) => .seq _ _ _ (.seq _ _ _ h₁ h₂) h₃
         ⟨mp, mpr⟩
 
-    theorem Command.identity_assignment {id: String}: (Command.assign id (.ident id)).equiv Command.skip
-      | s₁, s₂ =>
+    theorem Command.identity_assignment {id: String}: [Imp| <[var:id]> := <[id:id]>] ≈ [Imp| skip]
+      | _, _ =>
         -- Should use Maps.TotalMap.updateSame
-        have mp: CommandEval (.assign id id) s₁ s₂ → CommandEval .skip s₁ s₂
+        have mp
           | .assign _ h => sorry
-        have mpr: CommandEval .skip s₁ s₂ → CommandEval (.assign id id) s₁ s₂
+        have mpr
           | .skip _ => sorry
         ⟨mp, mpr⟩
 
-    theorem Command.assign_arith_equiv {id: String} {e: Arith} (h: (id: Arith).equiv e): Command.skip.equiv (Command.assign id e)
-      | s₁, s₂ =>
-        have mp: CommandEval .skip s₁ s₂ → CommandEval (.assign id e) s₁ s₂
+    theorem Command.assign_arith_equiv {id: String} {e: Arith} (h: [Arith| <[id:id]>] ≈ e): [Imp| skip] ≈ [Imp| <[var:id]> := <[arith:e]> ]
+      | _, _ =>
+        have mp
           | .skip _ => sorry
-        have mpr: CommandEval (.assign id e) s₁ s₂ → CommandEval .skip s₁ s₂
+        have mpr
           | .assign _ _ => sorry
         ⟨mp, mpr⟩
   end Term
 
   namespace Tactic
     @[scoped simp]
-    theorem Command.skip_left {c: Command}: (Command.seq .skip c).equiv c := by
+    theorem Command.skip_left {c: Command}: [Imp| skip; <[ c ]>] ≈ c := by
       intro s₁ s₂
       apply Iff.intro
       · intro
@@ -249,7 +251,7 @@ namespace SoftwareFoundations.ProgrammingLanguageFoundations.Equiv
             repeat assumption
 
     @[scoped simp]
-    theorem Command.skip_right {c: Command}: (Command.seq c .skip).equiv c := by
+    theorem Command.skip_right {c: Command}: [Imp| <[ c ]>; skip] ≈ c := by
       intro s₁ s₂
       apply Iff.intro
       · intro
@@ -271,7 +273,7 @@ namespace SoftwareFoundations.ProgrammingLanguageFoundations.Equiv
             repeat assumption
           · apply CommandEval.skip
 
-    example {t f: Command}: (Command.if .true t f).equiv t := by
+    example {t f: Command}: [Imp| ite (tru) { <[t]> } else { <[f]> }] ≈ t := by
       intro s₁ s₂
       apply Iff.intro
       · intro
@@ -296,7 +298,7 @@ namespace SoftwareFoundations.ProgrammingLanguageFoundations.Equiv
             repeat assumption
 
     @[scoped simp]
-    theorem Command.if_true {b: Logic} {c₁ c₂: Command} (h: b.equiv .true): (Command.if b c₁ c₂).equiv c₁ := by
+    theorem Command.if_true {b: Logic} {c₁ c₂: Command} (h: b ≈ .true): [Imp| ite (<[expr:b]>) { <[ c₁ ]> } else { <[ c₂ ]> }] ≈ c₁ := by
       intro s₁ s₂
       apply Iff.intro
       · intro
@@ -322,7 +324,7 @@ namespace SoftwareFoundations.ProgrammingLanguageFoundations.Equiv
             repeat assumption
 
     @[scoped simp]
-    theorem Command.if_false {b: Logic} {c₁ c₂: Command} (h: b.equiv .false): (Command.if b c₁ c₂).equiv c₂ := by
+    theorem Command.if_false {b: Logic} {c₁ c₂: Command} (h: b ≈ .false): [Imp| ite (<[expr:b]>) { <[ c₁ ]> } else { <[ c₂ ]> }] ≈ c₂ := by
       intro s₁ s₂
       apply Iff.intro
       · intro
@@ -347,14 +349,14 @@ namespace SoftwareFoundations.ProgrammingLanguageFoundations.Equiv
             . apply CommandEval.whileFalse
               repeat assumption
 
-    theorem Command.if_swap {b: Logic} {c₁ c₂: Command}: (Command.if b c₁ c₂).equiv (Command.if (.not b) c₂ c₁) := by
+    theorem Command.if_swap {b: Logic} {c₁ c₂: Command}: [Imp| ite (<[expr:b]>) { <[ c₁ ]> } else { <[ c₂ ]> }] ≈ [Imp| ite (!<[expr:b]>) { <[ c₂ ]> } else { <[ c₁ ]> }] := by
       intro s₁ s₂
       apply Iff.intro
       · sorry
       · sorry
 
     @[scoped simp]
-    theorem Command.while_false {c: Logic} {b: Command} (h: c.equiv .false): (Command.while c b).equiv Command.skip := by
+    theorem Command.while_false {c: Logic} {b: Command} (h: c ≈ .false): [Imp| while (<[expr:c]>) { <[b]> }] ≈ [Imp| skip] := by
       intro s₁ s₂
       apply Iff.intro
       · intro
@@ -368,7 +370,7 @@ namespace SoftwareFoundations.ProgrammingLanguageFoundations.Equiv
             · rw [h s₁]
 
     @[scoped simp]
-    theorem Command.while_true {c: Logic} {b: Command} (h: c.equiv .true): (Command.while c b).equiv (Command.while .true Command.skip) := by
+    theorem Command.while_true {c: Logic} {b: Command} (h: c ≈ .true): [Imp| while (<[expr:c]>) { <[b]> }] ≈ [Imp| while (tru) { skip }] := by
       intro s₁ s₂
       apply Iff.intro
       · intro
@@ -389,7 +391,7 @@ namespace SoftwareFoundations.ProgrammingLanguageFoundations.Equiv
           contradiction
         | whileFalse _ _ => simp_all
       where
-        nonterm {c: Logic} {b: Command} {s₁ s₂: State} (h: c.equiv .true): ¬(CommandEval (.while c b) s₁ s₂) := by
+        nonterm {c: Logic} {b: Command} {s₁ s₂: State} (h: c ≈ .true): ¬(s₁ =[[Imp| while (<[expr: c ]>) { <[ b ]> }]]=> s₂) := by
           intro
           | .whileTrue s₃ s₄ s₅ h₁ h₂ h₃ =>
             -- simp_all
@@ -397,7 +399,7 @@ namespace SoftwareFoundations.ProgrammingLanguageFoundations.Equiv
             sorry
           | .whileFalse _ _ => simp_all
 
-    theorem Command.loop_unrolling {c: Logic} {b: Command}: (Command.while c b).equiv (Command.if c (Command.seq b (Command.while c b)) .skip) := by
+    theorem Command.loop_unrolling {c: Logic} {b: Command}: [Imp| while (<[expr: c]>) { <[b]> }] ≈ [Imp| ite (<[expr:c]>) { <[b]>; while (<[expr:c]>) { <[b]> }} else { skip }] := by
       intro s₁ s₂
       apply Iff.intro
       · intro
@@ -416,7 +418,7 @@ namespace SoftwareFoundations.ProgrammingLanguageFoundations.Equiv
         | .ifFalse _ _ h₁ (.skip _) =>
           exact CommandEval.whileFalse _ h₁
 
-    theorem Command.seq_assoc {c₁ c₂ c₂: Command}: (Command.seq (Command.seq c₁ c₂) c₃).equiv (Command.seq c₁ (Command.seq c₂ c₃)) := by
+    theorem Command.seq_assoc {c₁ c₂ c₂: Command}: [Imp| (<[c₁]>; <[c₂]>); <[c₃]>] ≈ [Imp| <[c₁]>; (<[c₂]>; <[c₃]>)] := by
       intro s₁ s₂
       apply Iff.intro
       · intro
@@ -433,13 +435,13 @@ namespace SoftwareFoundations.ProgrammingLanguageFoundations.Equiv
                  repeat assumption)
 
     @[scoped simp]
-    theorem Command.identity_assignment {id: String}: (Command.assign id (.ident id)).equiv Command.skip := by
+    theorem Command.identity_assignment {id: String}: [Imp| <[var:id]> := <[id:id]>] ≈ [Imp| skip] := by
       intro s₁ s₂
       apply Iff.intro
       · sorry
       · sorry
 
-    theorem Command.assign_arith_equiv {id: String} {e: Arith} (h₁: (id: Arith).equiv e): Command.skip.equiv (Command.assign id e) := by
+    theorem Command.assign_arith_equiv {id: String} {e: Arith} (h: [Arith| <[id:id]>] ≈ e): [Imp| skip] ≈ [Imp| <[var:id]> := <[arith:e]> ] := by
       unfold Command.equiv
       intro s₁ s₂
       apply Iff.intro
@@ -449,11 +451,11 @@ namespace SoftwareFoundations.ProgrammingLanguageFoundations.Equiv
 
   namespace Blended
     @[scoped simp]
-    theorem Command.skip_left {c: Command}: (Command.seq .skip c).equiv c
-      | s₁, s₂ =>
-        have mp: CommandEval (Command.seq .skip c) s₁ s₂ → CommandEval c s₁ s₂
+    theorem Command.skip_left {c: Command}: [Imp| skip; <[ c ]>] ≈ c
+      | _, _ =>
+        have mp
           | .seq _ _ _ (.skip _) h₂ => h₂
-        have mpr: CommandEval c s₁ s₂ → CommandEval (Command.seq .skip c) s₁ s₂
+        have mpr
           | .skip _                   => .seq _ _ _ (.skip _) (.skip _)
           | .assign _ h               => .seq _ _ _ (.skip _) (.assign _ h)
           | .seq _ _ _ h₁ h₂          => .seq _ _ _ (.skip _) (.seq _ _ _ h₁ h₂)
@@ -464,11 +466,11 @@ namespace SoftwareFoundations.ProgrammingLanguageFoundations.Equiv
         ⟨mp, mpr⟩
 
     @[scoped simp]
-    theorem Command.skip_right {c: Command}: (Command.seq c .skip).equiv c
-      | s₁, s₂ =>
-        have mp: CommandEval (Command.seq c .skip) s₁ s₂ → CommandEval c s₁ s₂
+    theorem Command.skip_right {c: Command}: [Imp| <[ c ]>; skip] ≈ c
+      | _, _ =>
+        have mp
           | .seq _ _ _ h₁ (.skip _) => h₁
-        have mpr: CommandEval c s₁ s₂ → CommandEval (Command.seq c .skip) s₁ s₂
+        have mpr
           | .skip _                   => .seq _ _ _ (.skip _) (.skip _)
           | .assign _ h               => .seq _ _ _ (.assign _ h) (.skip _)
           | .seq _ _ _ h₁ h₂          => .seq _ _ _ (.seq _ _ _ h₁ h₂) (.skip _)
@@ -479,12 +481,12 @@ namespace SoftwareFoundations.ProgrammingLanguageFoundations.Equiv
         ⟨mp, mpr⟩
 
     @[scoped simp]
-    example {t f: Command}: (Command.if .true t f).equiv t
-      | s₁, s₂ =>
-        have mp: CommandEval (.if .true t f) s₁ s₂ → CommandEval t s₁ s₂
+    example {t f: Command}: [Imp| ite (tru) { <[t]> } else { <[f]> }] ≈ t
+      | _, _ =>
+        have mp
           | .ifTrue _ _ _ h₂ => h₂
           | .ifFalse _ _ h₁ _ => Logic.true.trueFalse rfl h₁
-        have mpr: CommandEval t s₁ s₂ → CommandEval (.if .true t f) s₁ s₂
+        have mpr
           | .skip _                   => .ifTrue _ _ rfl (.skip _)
           | .assign _ h               => .ifTrue _ _ rfl (.assign _ h)
           | .seq _ _ _ h₁ h₂          => .ifTrue _ _ rfl (.seq _ _ _ h₁ h₂)
@@ -495,153 +497,167 @@ namespace SoftwareFoundations.ProgrammingLanguageFoundations.Equiv
         ⟨mp, mpr⟩
 
     @[scoped simp]
-    theorem Command.if_true {b: Logic} {c₁ c₂: Command} (h: b.equiv .true): (Command.if b c₁ c₂).equiv c₁
-      | s₁, s₂ =>
-        have tru: b.eval s₁ = Logic.true.eval s₁ := h _
-        have mp: CommandEval (.if b c₁ c₂) s₁ s₂ → CommandEval c₁ s₁ s₂
+    theorem Command.if_true {b: Logic} {c₁ c₂: Command} (h: b ≈ .true): [Imp| ite (<[expr:b]>) { <[ c₁ ]> } else { <[ c₂ ]> }] ≈ c₁
+      | _, _ =>
+        have truu: b.eval _ = Logic.true.eval _ := h _
+        have mp
           | .ifTrue _ _ _ h₂ => h₂
-          | .ifFalse _ _ h₁ _ => b.trueFalse tru h₁
-        have mpr: CommandEval c₁ s₁ s₂ → CommandEval (.if b c₁ c₂) s₁ s₂
-          | .skip _                   => .ifTrue _ _ tru (.skip _)
-          | .assign _ h₁              => .ifTrue _ _ tru (.assign _ h₁)
-          | .seq _ _ _ h₁ h₂          => .ifTrue _ _ tru (.seq _ _ _ h₁ h₂)
-          | .ifTrue _ _ h₁ h₂         => .ifTrue _ _ tru (.ifTrue _ _ h₁ h₂)
-          | .ifFalse _ _ h₁ h₂        => .ifTrue _ _ tru (.ifFalse _ _ h₁ h₂)
-          | .whileTrue _ _ _ h₁ h₂ h₃ => .ifTrue _ _ tru (.whileTrue _ _ _ h₁ h₂ h₃)
-          | .whileFalse _ h₁          => .ifTrue _ _ tru (.whileFalse _ h₁)
+          | .ifFalse _ _ h₁ _ => b.trueFalse truu h₁
+        have mpr
+          | .skip _                   => .ifTrue _ _ truu (.skip _)
+          | .assign _ h₁              => .ifTrue _ _ truu (.assign _ h₁)
+          | .seq _ _ _ h₁ h₂          => .ifTrue _ _ truu (.seq _ _ _ h₁ h₂)
+          | .ifTrue _ _ h₁ h₂         => .ifTrue _ _ truu (.ifTrue _ _ h₁ h₂)
+          | .ifFalse _ _ h₁ h₂        => .ifTrue _ _ truu (.ifFalse _ _ h₁ h₂)
+          | .whileTrue _ _ _ h₁ h₂ h₃ => .ifTrue _ _ truu (.whileTrue _ _ _ h₁ h₂ h₃)
+          | .whileFalse _ h₁          => .ifTrue _ _ truu (.whileFalse _ h₁)
         ⟨mp, mpr⟩
 
     @[scoped simp]
-    theorem Command.if_false {b: Logic} {c₁ c₂: Command} (h: b.equiv .false): (Command.if b c₁ c₂).equiv c₂
-      | s₁, s₂ =>
-        have fls: b.eval s₁ = Logic.false.eval s₁ := h _
-        have mp: CommandEval (.if b c₁ c₂) s₁ s₂ → CommandEval c₂ s₁ s₂
-          | .ifTrue _ _ h₁ _ => b.trueFalse h₁ fls
+    theorem Command.if_false {b: Logic} {c₁ c₂: Command} (h: b ≈ .false): [Imp| ite (<[expr:b]>) { <[ c₁ ]> } else { <[ c₂ ]> }] ≈ c₂
+      | _, _ =>
+        have falz: b.eval _ = Logic.false.eval _ := h _
+        have mp
+          | .ifTrue _ _ h₁ _ => b.trueFalse h₁ falz
           | .ifFalse _ _ _ h₂ => h₂
-        have mpr: CommandEval c₂ s₁ s₂ → CommandEval (.if b c₁ c₂) s₁ s₂
-          | .skip _                   => .ifFalse _ _ fls (.skip _)
-          | .assign _ h₁              => .ifFalse _ _ fls (.assign _ h₁)
-          | .seq _ _ _ h₁ h₂          => .ifFalse _ _ fls (.seq _ _ _ h₁ h₂)
-          | .ifTrue _ _ h₁ h₂         => .ifFalse _ _ fls (.ifTrue _ _ h₁ h₂)
-          | .ifFalse _ _ h₁ h₂        => .ifFalse _ _ fls (.ifFalse _ _ h₁ h₂)
-          | .whileTrue _ _ _ h₁ h₂ h₃ => .ifFalse _ _ fls (.whileTrue _ _ _ h₁ h₂ h₃)
-          | .whileFalse _ h₁          => .ifFalse _ _ fls (.whileFalse _ h₁)
+        have mpr
+          | .skip _                   => .ifFalse _ _ falz (.skip _)
+          | .assign _ h₁              => .ifFalse _ _ falz (.assign _ h₁)
+          | .seq _ _ _ h₁ h₂          => .ifFalse _ _ falz (.seq _ _ _ h₁ h₂)
+          | .ifTrue _ _ h₁ h₂         => .ifFalse _ _ falz (.ifTrue _ _ h₁ h₂)
+          | .ifFalse _ _ h₁ h₂        => .ifFalse _ _ falz (.ifFalse _ _ h₁ h₂)
+          | .whileTrue _ _ _ h₁ h₂ h₃ => .ifFalse _ _ falz (.whileTrue _ _ _ h₁ h₂ h₃)
+          | .whileFalse _ h₁          => .ifFalse _ _ falz (.whileFalse _ h₁)
         ⟨mp, mpr⟩
 
-    theorem Command.if_swap {b: Logic} {c₁ c₂: Command}: (Command.if b c₁ c₂).equiv (Command.if (.not b) c₂ c₁) := by sorry
+    theorem Command.if_swap {b: Logic} {c₁ c₂: Command}: [Imp| ite (<[expr:b]>) { <[ c₁ ]> } else { <[ c₂ ]> }] ≈ [Imp| ite (!<[expr:b]>) { <[ c₂ ]> } else { <[ c₁ ]> }] := sorry
 
     @[scoped simp]
-    theorem Command.while_false {c: Logic} {b: Command} (h: c.equiv .false): (Command.while c b).equiv Command.skip
-      | s₁, s₂ =>
-        have fls: c.eval s₁ = Logic.false.eval s₁ := h _
-        have mp: CommandEval (.while c b) s₁ s₂ → CommandEval .skip s₁ s₂
-          | .whileTrue _ _ _ h₁ _ _=> c.trueFalse h₁ fls
+    theorem Command.while_false {c: Logic} {b: Command} (h: c ≈ .false): [Imp| while (<[expr:c]>) { <[b]> }] ≈ [Imp| skip]
+      | _, _ =>
+        have falz: c.eval _ = Logic.false.eval _ := h _
+        have mp
+          | .whileTrue _ _ _ h₁ _ _=> c.trueFalse h₁ falz
           | .whileFalse _ _ => .skip _
-        have mpr: CommandEval .skip s₁ s₂ → CommandEval (.while c b) s₁ s₂
-          | .skip _ => .whileFalse _ fls
+        have mpr
+          | .skip _ => .whileFalse _ falz
         ⟨mp, mpr⟩
 
     @[scoped simp]
-    theorem Command.while_true {c: Logic} {b: Command} (h: c.equiv .true): (Command.while c b).equiv (Command.while .true Command.skip)
-      | s₁, s₂ =>
-        have tru: c.eval s₁ = Logic.true.eval s₁ := h _
+    theorem Command.while_true {c: Logic} {b: Command} (h: c ≈ .true): [Imp| while (<[expr:c]>) { <[b]> }] ≈ [Imp| while (tru) { skip }]
+      | _, _ =>
+        have truu: c.eval _ = Logic.true.eval _ := h _
         have hh: Logic.true.equiv .true
           | _ => rfl
-        have mp: CommandEval (.while c b) s₁ s₂ → CommandEval (.while .true .skip) s₁ s₂
+        have mp
           | .whileTrue _ _ _ h₁ h₂ h₃ => absurd (CommandEval.whileTrue _ _ _ h₁ h₂ h₃) (nonterm h)
-          | .whileFalse _ h₁ => c.trueFalse tru h₁
-        have mpr: CommandEval (.while .true .skip) s₁ s₂ → CommandEval (.while c b) s₁ s₂
+          | .whileFalse _ h₁ => c.trueFalse truu h₁
+        have mpr
           | .whileTrue _ _ _ h₁ h₂ h₃ => absurd (CommandEval.whileTrue _ _ _ h₁ h₂ h₃) (nonterm hh)
           | .whileFalse _ h₁ => Logic.true.trueFalse rfl h₁
         ⟨mp, mpr⟩
       where
-        nonterm {c: Logic} {b: Command} {s₁ s₂: State} (h: c.equiv .true): ¬(CommandEval (.while c b) s₁ s₂)
+        nonterm {c: Logic} {b: Command} {s₁ s₂: State} (h: c ≈ .true): ¬(s₁ =[[Imp| while (<[expr: c ]>) { <[ b ]> }]]=> s₂)
           | .whileTrue _ _ _ _ _ h₃ => sorry
           | .whileFalse _ h₁ => c.trueFalse (h _) h₁
 
-    theorem Command.loop_unrolling {c: Logic} {b: Command}: (Command.while c b).equiv (Command.if c (Command.seq b (Command.while c b)) .skip)
-      | s₁, s₂ =>
-        have mp: CommandEval (.while c b) s₁ s₂ → CommandEval (.if c (.seq b (.while c b)) .skip) s₁ s₂
+    theorem Command.loop_unrolling {c: Logic} {b: Command}: [Imp| while (<[expr:c]>) { <[b]> }] ≈ [Imp| ite (<[expr:c]>) { <[b]>; while (<[expr:c]>) { <[b]> }} else { skip }]
+      | _, _ =>
+        have mp
           | .whileTrue _ _ _ h₁ h₂ h₃ => .ifTrue _ _ h₁ (.seq _ _ _ h₂ h₃)
           | .whileFalse _ h₁ => .ifFalse _ _ h₁ (.skip _)
-        have mpr: CommandEval (.if c (.seq b (.while c b)) .skip) s₁ s₂ → CommandEval (.while c b) s₁ s₂
+        have mpr
           | .ifTrue _ _ h₁ (.seq _ _ _ h₂ h₃) => .whileTrue _ _ _ h₁ h₂ h₃
           | .ifFalse _ _ h₁ (.skip _) => .whileFalse _ h₁
         ⟨mp, mpr⟩
 
-    theorem Command.seq_assoc {c₁ c₂ c₃: Command}: (Command.seq (Command.seq c₁ c₂) c₃).equiv (Command.seq c₁ (Command.seq c₂ c₃))
-      | s₁, s₂ =>
-        have mp: CommandEval (.seq (.seq c₁ c₂) c₃) s₁ s₂ → CommandEval (.seq c₁ (.seq c₂ c₃)) s₁ s₂
+    theorem Command.seq_assoc {c₁ c₂ c₃: Command}: [Imp| (<[c₁]>; <[c₂]>); <[c₃]>] ≈ [Imp| <[c₁]>; (<[c₂]>; <[c₃]>)]
+      | _, _ =>
+        have mp
           | .seq _ _ _ (.seq _ _ _ h₁ h₂) h₃ => .seq _ _ _ h₁ (.seq _ _ _ h₂ h₃)
-        have mpr: CommandEval (.seq c₁ (.seq c₂ c₃)) s₁ s₂ → CommandEval (.seq (.seq c₁ c₂) c₃) s₁ s₂
+        have mpr
           | .seq _ _ _ h₁ (.seq _ _ _ h₂ h₃) => .seq _ _ _ (.seq _ _ _ h₁ h₂) h₃
         ⟨mp, mpr⟩
 
     @[scoped simp]
-    theorem Command.identity_assignment {id: String}: (Command.assign id (.ident id)).equiv Command.skip := by sorry
+    theorem Command.identity_assignment {id: String}: [Imp| <[var:id]> := <[id:id]>] ≈ [Imp| skip] := by sorry
 
-    theorem Command.assign_arith_equiv {id: String} {e: Arith} (h₁: (id: Arith).equiv e): Command.skip.equiv (Command.assign id e) := by sorry
+    theorem Command.assign_arith_equiv {id: String} {e: Arith} (h: [Arith| <[id:id]>] ≈ e): [Imp| skip] ≈ [Imp| <[var:id]> := <[arith:e]> ] := by sorry
   end Blended
 
   section
     -- Diverges: X starts > 1 and only increases.
-    private def a: Command :=
-      .while (.gt "X" 0)
-        (.assign "X" ("X" + 1))
+    private def a := [Imp|
+      while (X > 0) {
+        X := X + 1
+      }
+    ]
 
     -- Terminates:
     -- If X == 0, then X := 0, Y := 0
     -- If X != 0, then X := X, Y := 0
     -- In both cases, X retains its value and Y := 0
-    private def b: Command :=
-      .seq
-        (.if (.eq "X" 0)
-          (.seq                     -- true: X := 1, Y := 1
-            (.assign "X" ("X" + 1))
-            (.assign "Y" 1))
-          (.assign "Y" 0))          -- false: X != 0, Y := 0
-        (.seq
-          (.assign "X" ("X" - "Y")) -- true: X := 0, false: X := X
-          (.assign "Y" 0))          -- true: Y := 0, false: Y := 0
+    private def b := [Imp|
+      ite (X = 0) {
+        X := X + 1;
+        Y := 1
+      } else {
+        Y := 0
+      };
+      X := X - Y;
+      Y := 0
+    ]
 
     -- Terminates, no-op
-    private def c: Command :=
-      .skip
+    private def c := [Imp|
+      skip
+    ]
 
     -- Diverges: X is positive (Nat ≠ 0). X * positive is ≥ 0, + 1 > 0.
-    private def d: Command :=
-      .while (.neq "X" 0)
-        (.assign "X" ("X" * "Y" + 1))
+    private def d := [Imp|
+      while (X ≠ 0) {
+        X := X * Y + 1
+      }
+    ]
 
     -- After termination, Y := 0 and, implicitly, X := X
-    private def e: Command :=
-      .assign "Y" 0
+    private def e := [Imp|
+      Y := 0
+    ]
 
     -- Diverges: Y := X + 1, so X != Y.  In the loop, assigns the same, so loop
     -- never terminates.
-    private def f: Command :=
-      .seq
-        (.assign "Y" ("X" + 1))
-        (.while (.neq "X" "Y")
-          (.assign "Y" ("X" + 1)))
+    private def f := [Imp|
+      Y := X + 1;
+      while (X ≠ Y) {
+        Y := X + 1
+      }
+    ]
 
     -- Diverges: Canonical example
-    private def g: Command :=
-      .while .true .skip
+    private def g := [Imp|
+      while (tru) {
+        skip
+      }
+    ]
 
     -- No-op.  X always equals X, so is "while false"
-    private def h: Command :=
-      .while (.neq "X" "X")
-        (.assign "X" ("X" + 1))
+    private def h := [Imp|
+      while (X ≠ X) {
+        X := X + 1
+      }
+    ]
 
     -- May diverge:
     -- * If X = Y, terminates.
     -- * If X != Y, X will never equal Y.
-    private def i: Command :=
-      .while (.neq "X" "Y")
-        (.assign "X" ("Y" + 1))
+    private def i := [Imp|
+      while (X ≠ Y) {
+        X := Y + 1
+      }
+    ]
 
-    private def equiv_classes: List (List Command) := [
+    private def equiv_classes := [
       -- Diverges
       [a, d, f, g],
       -- X is retained, Y := 0
@@ -652,40 +668,40 @@ namespace SoftwareFoundations.ProgrammingLanguageFoundations.Equiv
       [i]
     ]
 
-    example: a.equiv d
-      | s₁, s₂ =>
-        have mp: CommandEval a s₁ s₂ → CommandEval d s₁ s₂ := sorry
-        have mpr: CommandEval d s₁ s₂ → CommandEval a s₁ s₂ := sorry
+    example: a ≈ d
+      | _, _ =>
+        have mp := sorry
+        have mpr := sorry
         ⟨mp, mpr⟩
-    example: d.equiv f
-      | s₁, s₂ =>
-        have mp: CommandEval d s₁ s₂ → CommandEval f s₁ s₂ := sorry
-        have mpr: CommandEval f s₁ s₂ → CommandEval d s₁ s₂ := sorry
+    example: d ≈ f
+      | _, _ =>
+        have mp := sorry
+        have mpr := sorry
         ⟨mp, mpr⟩
-    example: f.equiv g
-      | s₁, s₂ =>
-        have mp: CommandEval f s₁ s₂ → CommandEval g s₁ s₂ := sorry
-        have mpr: CommandEval g s₁ s₂ → CommandEval f s₁ s₂ := sorry
-        ⟨mp, mpr⟩
-
-    example: b.equiv e
-      | s₁, s₂ =>
-        have mp: CommandEval b s₁ s₂ → CommandEval e s₁ s₂ := sorry
-        have mpr: CommandEval e s₁ s₂ → CommandEval b s₁ s₂ := sorry
+    example: f ≈ g
+      | _, _ =>
+        have mp := sorry
+        have mpr := sorry
         ⟨mp, mpr⟩
 
-    example: c.equiv h
-      | s₁, s₂ =>
-        have mp: CommandEval c s₁ s₂ → CommandEval h s₁ s₂ := sorry
-        have mpr: CommandEval h s₁ s₂ → CommandEval c s₁ s₂ := sorry
+    example: b ≈ e
+      | _, _ =>
+        have mp := sorry
+        have mpr := sorry
         ⟨mp, mpr⟩
 
-    example: ¬(a.equiv b) := sorry
-    example: ¬(a.equiv c) := sorry
-    example: ¬(a.equiv i) := sorry
-    example: ¬(b.equiv c) := sorry
-    example: ¬(b.equiv i) := sorry
-    example: ¬(c.equiv i) := sorry
+    example: c ≈ h
+      | _, _ =>
+        have mp := sorry
+        have mpr := sorry
+        ⟨mp, mpr⟩
+
+    example: ¬(a ≈ b) := sorry
+    example: ¬(a ≈ c) := sorry
+    example: ¬(a ≈ i) := sorry
+    example: ¬(b ≈ c) := sorry
+    example: ¬(b ≈ i) := sorry
+    example: ¬(c ≈ i) := sorry
 
     -- By transitivity (below) this proves the equivalence classes
   end
@@ -699,80 +715,80 @@ namespace SoftwareFoundations.ProgrammingLanguageFoundations.Equiv
   -/
 
   namespace Term
-    theorem Arith.equiv.refl {e: Arith}: e.equiv e
+    theorem Arith.equiv.refl {e: Arith}: e ≈ e
       | _ => Eq.refl (e.eval _)
-    theorem Arith.equiv.symm {e₁ e₂: Arith} (h: e₁.equiv e₂): e₂.equiv e₁
+    theorem Arith.equiv.symm {e₁ e₂: Arith} (h: e₁ ≈ e₂): e₂ ≈ e₁
       | _ => Eq.symm (h _)
-    theorem Arith.equiv.trans {e₁ e₂ e₃: Arith} (h₁: e₁.equiv e₂) (h₂: e₂.equiv e₃): e₁.equiv e₃
+    theorem Arith.equiv.trans {e₁ e₂ e₃: Arith} (h₁: e₁ ≈ e₂) (h₂: e₂ ≈ e₃): e₁ ≈ e₃
       | _ => Eq.trans (h₁ _) (h₂ _)
 
-    theorem Logic.equiv.refl {b: Logic}: b.equiv b
+    theorem Logic.equiv.refl {b: Logic}: b ≈ b
       | _ => Eq.refl (b.eval _)
-    theorem Logic.equiv.symm {b₁ b₂: Logic} (h: b₁.equiv b₂): b₂.equiv b₁
+    theorem Logic.equiv.symm {b₁ b₂: Logic} (h: b₁ ≈ b₂): b₂ ≈ b₁
       | _ => Eq.symm (h _)
-    theorem Logic.equiv.trans {b₁ b₂ b₃: Logic} (h₁: b₁.equiv b₂) (h₂: b₂.equiv b₃): b₁.equiv b₃
+    theorem Logic.equiv.trans {b₁ b₂ b₃: Logic} (h₁: b₁ ≈ b₂) (h₂: b₂ ≈ b₃): b₁ ≈ b₃
       | _ => Eq.trans (h₁ _) (h₂ _)
 
-    theorem Command.equiv.refl {c: Command}: c.equiv c
+    theorem Command.equiv.refl {c: Command}: c ≈ c
       | _, _ => Iff.refl (CommandEval c _ _)
-    theorem Command.equiv.symm {c₁ c₂: Command} (h: c₁.equiv c₂): c₂.equiv c₁
+    theorem Command.equiv.symm {c₁ c₂: Command} (h: c₁ ≈ c₂): c₂ ≈ c₁
       | _, _ => Iff.symm (h _ _)
-    theorem Command.equiv.trans {c₁ c₂ c₃: Command} (h₁: c₁.equiv c₂) (h₂: c₂.equiv c₃): c₁.equiv c₃
+    theorem Command.equiv.trans {c₁ c₂ c₃: Command} (h₁: c₁ ≈ c₂) (h₂: c₂ ≈ c₃): c₁ ≈ c₃
       | _, _ => Iff.trans (h₁ _ _) (h₂ _ _)
   end Term
 
   namespace Tactic
-    theorem Arith.equiv.refl {e: Arith}: e.equiv e := by
+    theorem Arith.equiv.refl {e: Arith}: e ≈ e := by
       intro
       rfl
-    theorem Arith.equiv.symm {e₁ e₂: Arith} (h: e₁.equiv e₂): e₂.equiv e₁ := by
+    theorem Arith.equiv.symm {e₁ e₂: Arith} (h: e₁ ≈ e₂): e₂ ≈ e₁ := by
       intro
       rw [h _]
-    theorem Arith.equiv.trans {e₁ e₂ e₃: Arith} (h₁: e₁.equiv e₂) (h₂: e₂.equiv e₃): e₁.equiv e₃ := by
+    theorem Arith.equiv.trans {e₁ e₂ e₃: Arith} (h₁: e₁ ≈ e₂) (h₂: e₂ ≈ e₃): e₁ ≈ e₃ := by
       intro
       rw [h₁ _, h₂ _]
 
-    theorem Logic.equiv.refl {b: Logic}: b.equiv b := by
+    theorem Logic.equiv.refl {b: Logic}: b ≈ b := by
       intro
       rfl
-    theorem Logic.equiv.symm {b₁ b₂: Logic} (h: b₁.equiv b₂): b₂.equiv b₁ := by
+    theorem Logic.equiv.symm {b₁ b₂: Logic} (h: b₁ ≈ b₂): b₂ ≈ b₁ := by
       intro
       rw [h _]
-    theorem Logic.equiv.trans {b₁ b₂ b₃: Logic} (h₁: b₁.equiv b₂) (h₂: b₂.equiv b₃): b₁.equiv b₃ := by
+    theorem Logic.equiv.trans {b₁ b₂ b₃: Logic} (h₁: b₁ ≈ b₂) (h₂: b₂ ≈ b₃): b₁ ≈ b₃ := by
       intro
       rw [h₁ _, h₂ _]
 
-    theorem Command.equiv.refl {c: Command}: c.equiv c := by
+    theorem Command.equiv.refl {c: Command}: c ≈ c := by
       intro _ _
       rfl
-    theorem Command.equiv.symm {c₁ c₂: Command} (h: c₁.equiv c₂): c₂.equiv c₁ := by
+    theorem Command.equiv.symm {c₁ c₂: Command} (h: c₁ ≈ c₂): c₂ ≈ c₁ := by
       intro _ _
       rw [h _ _]
-    theorem Command.equiv.trans {c₁ c₂ c₃: Command} (h₁: c₁.equiv c₂) (h₂: c₂.equiv c₃): c₁.equiv c₃ := by
+    theorem Command.equiv.trans {c₁ c₂ c₃: Command} (h₁: c₁ ≈ c₂) (h₂: c₂ ≈ c₃): c₁ ≈ c₃ := by
       intro _ _
       rw [h₁ _ _, h₂ _ _]
   end Tactic
 
   namespace Blended
-    theorem Arith.equiv.refl {e: Arith}: e.equiv e
+    theorem Arith.equiv.refl {e: Arith}: e ≈ e
       | _ => Eq.refl (e.eval _)
-    theorem Arith.equiv.symm {e₁ e₂: Arith} (h: e₁.equiv e₂): e₂.equiv e₁
+    theorem Arith.equiv.symm {e₁ e₂: Arith} (h: e₁ ≈ e₂): e₂ ≈ e₁
       | _ => Eq.symm (h _)
-    theorem Arith.equiv.trans {e₁ e₂ e₃: Arith} (h₁: e₁.equiv e₂) (h₂: e₂.equiv e₃): e₁.equiv e₃
+    theorem Arith.equiv.trans {e₁ e₂ e₃: Arith} (h₁: e₁ ≈ e₂) (h₂: e₂ ≈ e₃): e₁ ≈ e₃
       | _ => Eq.trans (h₁ _) (h₂ _)
 
-    theorem Logic.equiv.refl {b: Logic}: b.equiv b
+    theorem Logic.equiv.refl {b: Logic}: b ≈ b
       | _ => Eq.refl (b.eval _)
-    theorem Logic.equiv.symm {b₁ b₂: Logic} (h: b₁.equiv b₂): b₂.equiv b₁
+    theorem Logic.equiv.symm {b₁ b₂: Logic} (h: b₁ ≈ b₂): b₂ ≈ b₁
       | _ => Eq.symm (h _)
-    theorem Logic.equiv.trans {b₁ b₂ b₃: Logic} (h₁: b₁.equiv b₂) (h₂: b₂.equiv b₃): b₁.equiv b₃
+    theorem Logic.equiv.trans {b₁ b₂ b₃: Logic} (h₁: b₁ ≈ b₂) (h₂: b₂ ≈ b₃): b₁ ≈ b₃
       | _ => Eq.trans (h₁ _) (h₂ _)
 
-    theorem Command.equiv.refl {c: Command}: c.equiv c
+    theorem Command.equiv.refl {c: Command}: c ≈ c
       | _, _ => Iff.refl (CommandEval c _ _)
-    theorem Command.equiv.symm {c₁ c₂: Command} (h: c₁.equiv c₂): c₂.equiv c₁
+    theorem Command.equiv.symm {c₁ c₂: Command} (h: c₁ ≈ c₂): c₂ ≈ c₁
       | _, _ => Iff.symm (h _ _)
-    theorem Command.equiv.trans {c₁ c₂ c₃: Command} (h₁: c₁.equiv c₂) (h₂: c₂.equiv c₃): c₁.equiv c₃
+    theorem Command.equiv.trans {c₁ c₂ c₃: Command} (h₁: c₁ ≈ c₂) (h₂: c₂ ≈ c₃): c₁ ≈ c₃
       | _, _ => Iff.trans (h₁ _ _) (h₂ _ _)
   end Blended
 
@@ -780,27 +796,31 @@ namespace SoftwareFoundations.ProgrammingLanguageFoundations.Equiv
   ### Behavioral Equivalence is a Congruence
   -/
 
-  private def congr_prog₁: Command :=
-    .seq
-      (.assign "X" 0)
-      (.if (.eq "X" 0)
-        (.assign "Y" 0)
-        (.assign "Y" 42))
+  private def congr_prog₁ := [Imp|
+    X := 0;
+    ite (X = 0) {
+      Y := 0
+    } else {
+      Y := 42
+    }
+  ]
 
-  private def congr_prog₂: Command :=
-    .seq
-      (.assign "X" 0)
-      (.if (.eq "X" 0)
-        (.assign "Y" ("X" - "X"))
-        (.assign "Y" 42))
+  private def congr_prog₂ := [Imp|
+    X := 0;
+    ite (X = 0) {
+      Y := X - X
+    } else {
+      Y := 42
+    }
+  ]
 
   namespace Term
-    theorem Command.skip.congr: Command.skip.equiv .skip
+    theorem Command.skip.congr: [Imp| skip] ≈ [Imp| skip]
       | _, _ => Iff.refl _
 
-    theorem Command.assign.congr {id: String} {e₁ e₂: Arith} (h₁: e₁.equiv e₂): (Command.assign id e₁).equiv (.assign id e₂)
+    theorem Command.assign.congr {id: String} {e₁ e₂: Arith} (h₁: e₁ ≈ e₂): [Imp| <[var:id]> := <[arith:e₁]> ].equiv [Imp| <[var:id]> := <[arith:e₂]>]
       | s₁, s₂ =>
-        have h {id: String} {e₁ e₂: Arith} (h: e₁.equiv e₂): CommandEval (.assign id e₁) s₁ s₂ → CommandEval (.assign id e₂) s₁ s₂
+        have h {id: String} {e₁ e₂: Arith} (h: e₁ ≈ e₂): (s₁ =[[Imp| <[var:id]> := <[arith:e₁]>]]=> s₂) → s₁ =[[Imp| <[var:id]> := <[arith:e₂]>]]=> s₂
           | .assign _ h₁ =>
             have h₂: e₂.eval _ = _ :=
               calc e₂.eval _
@@ -810,14 +830,14 @@ namespace SoftwareFoundations.ProgrammingLanguageFoundations.Equiv
         have h₂ := Arith.equiv.symm h₁
         ⟨h h₁, h h₂⟩
 
-    theorem Command.seq.congr {c₁ c₂ c₃ c₄: Command} (h₁: c₁.equiv c₂) (h₂: c₃.equiv c₄): (Command.seq c₁ c₃).equiv (.seq c₂ c₄)
+    theorem Command.seq.congr {c₁ c₂ c₃ c₄: Command} (h₁: c₁ ≈ c₂) (h₂: c₃ ≈ c₄): [Imp| <[c₁]>; <[c₃]>] ≈ [Imp| <[c₂]>; <[c₄]>]
       | s₁, s₂ =>
-        have h {c₁ c₂ c₃ c₄: Command} (h₁: c₁.equiv c₂) (h₂: c₃.equiv c₄): CommandEval (.seq c₁ c₃) s₁ s₂ → CommandEval (.seq c₂ c₄) s₁ s₂
+        have h {c₁ c₂ c₃ c₄: Command} (h₁: c₁ ≈ c₂) (h₂: c₃ ≈ c₄): (s₁ =[[Imp| <[c₁]>; <[c₃]>]]=> s₂) → s₁ =[[Imp| <[c₂]>; <[c₄]>]]=> s₂
           | .seq _ _ _ h₃ h₄ =>
-            have h₅: CommandEval c₂ _ _ :=
+            have h₅: _ =[c₂]=> _ :=
               have ⟨h, _⟩ := h₁ _ _
               h h₃
-            have h₆: CommandEval c₄ _ _ :=
+            have h₆: _ =[c₄]=> _ :=
               have ⟨h, _⟩ := h₂ _ _
               h h₄
             .seq _ _ _ h₅ h₆
@@ -825,9 +845,9 @@ namespace SoftwareFoundations.ProgrammingLanguageFoundations.Equiv
         have h₄ := Command.equiv.symm h₂
         ⟨h h₁ h₂, h h₃ h₄⟩
 
-    theorem Command.if.congr {c₁ c₂: Logic} {t₁ t₂ f₁ f₂: Command} (h₁: c₁.equiv c₂) (h₂: t₁.equiv t₂) (h₃: f₁.equiv f₂): (Command.if c₁ t₁ f₁).equiv (.if c₂ t₂ f₂)
+    theorem Command.if.congr {c₁ c₂: Logic} {t₁ t₂ f₁ f₂: Command} (h₁: c₁ ≈ c₂) (h₂: t₁ ≈ t₂) (h₃: f₁ ≈ f₂): [Imp| ite (<[expr:c₁]>) { <[t₁]> } else { <[f₁]> }] ≈ [Imp| ite (<[expr:c₂]>) { <[t₂]> } else { <[f₂]> }]
       | s₁, s₂ =>
-        have h {c₁ c₂: Logic} {t₁ t₂ f₁ f₂: Command} (h₁: c₁.equiv c₂) (h₂: t₁.equiv t₂) (h₃: f₁.equiv f₂): CommandEval (.if c₁ t₁ f₁) s₁ s₂ → CommandEval (.if c₂ t₂ f₂) s₁ s₂
+        have h {c₁ c₂: Logic} {t₁ t₂ f₁ f₂: Command} (h₁: c₁ ≈ c₂) (h₂: t₁ ≈ t₂) (h₃: f₁ ≈ f₂): (s₁ =[[Imp| ite (<[expr:c₁]>) { <[t₁]> } else { <[f₁]> }]]=> s₂) → s₁ =[[Imp| ite (<[expr:c₂]>) { <[t₂]> } else { <[f₂]> }]]=> s₂
           | .ifTrue _ _ h₄ h₅ =>
             have h₆: c₂.eval _ = true :=
               calc c₂.eval _
@@ -851,18 +871,18 @@ namespace SoftwareFoundations.ProgrammingLanguageFoundations.Equiv
         have h₆ := Command.equiv.symm h₃
         ⟨h h₁ h₂ h₃, h h₄ h₅ h₆⟩
 
-    theorem Command.while.congr {c₁ c₂: Logic} {b₁ b₂: Command} (h₁: c₁.equiv c₂) (h₂: b₁.equiv b₂): (Command.while c₁ b₁).equiv (.while c₂ b₂)
+    theorem Command.while.congr {c₁ c₂: Logic} {b₁ b₂: Command} (h₁: c₁ ≈ c₂) (h₂: b₁ ≈ b₂): [Imp| while (<[expr:c₁]>) { <[b₁]> }] ≈ [Imp| while (<[expr:c₂]>) { <[b₂]> }]
       | s₁, s₂ =>
-        have h {c₁ c₂: Logic} {b₁ b₂: Command} (h₁: c₁.equiv c₂) (h₂: b₁.equiv b₂): CommandEval (.while c₁ b₁) s₁ s₂ → CommandEval (.while c₂ b₂) s₁ s₂
+        have h {c₁ c₂: Logic} {b₁ b₂: Command} (h₁: c₁ ≈ c₂) (h₂: b₁ ≈ b₂): (s₁ =[[Imp| while (<[expr:c₁]>) { <[b₁]> }]]=> s₂) → s₁ =[[Imp| while (<[expr:c₂]>) { <[b₂]> }]]=> s₂
           | .whileTrue _ _ _ h₄ h₅ h₆ =>
             have h₇: c₂.eval _ = true :=
               calc c₂.eval _
                  _ = c₁.eval _ := Logic.equiv.symm h₁ _
                  _ = true      := h₄
-            have h₈: CommandEval b₂ _ _ :=
+            have h₈: _ =[b₂]=> _ :=
               have ⟨h, _⟩ := h₂ _ _
               h h₅
-            have h₉: CommandEval (.while c₂ b₂) _ _ :=
+            have h₉: _ =[[Imp| while (<[expr:c₂]>) { <[b₂]> }]]=> _ :=
               -- have h₁ := h₁ _
               -- have ⟨h₁, _⟩ := h₂ _ _
               -- h₆ h₁ h₂
@@ -878,25 +898,25 @@ namespace SoftwareFoundations.ProgrammingLanguageFoundations.Equiv
         have h₄ := Command.equiv.symm h₂
         ⟨h h₁ h₂, h h₃ h₄⟩
 
-    example: congr_prog₁.equiv congr_prog₂
-      | s₁, s₂ =>
-        have mp: CommandEval congr_prog₁ s₁ s₂ → CommandEval congr_prog₂ s₁ s₂
+    example: congr_prog₁ ≈ congr_prog₂
+      | _, _ =>
+        have mp
           | .seq _ _ _ _ (.ifTrue _ _ _ (.assign _ _)) => sorry
           | .seq _ _ _ _ (.ifFalse _ _ _ (.assign _ _)) => sorry
-        have mpr: CommandEval congr_prog₂ s₁ s₂ → CommandEval congr_prog₁ s₁ s₂
+        have mpr
           | .seq _ _ _ _ (.ifTrue _ _ _ (.assign _ _)) => sorry
           | .seq _ _ _ _ (.ifFalse _ _ _ (.assign _ _)) => sorry
         ⟨mp, mpr⟩
   end Term
 
   namespace Tactic
-    theorem Command.skip.congr: Command.skip.equiv .skip := by
+    theorem Command.skip.congr: [Imp| skip] ≈ [Imp| skip] := by
       intro s₁ s₂
       apply Iff.refl
 
-    theorem Command.assign.congr {id: String} {e₁ e₂: Arith} (h₁: e₁.equiv e₂): (Command.assign id e₁).equiv (.assign id e₂) := by
+    theorem Command.assign.congr {id: String} {e₁ e₂: Arith} (h₁: e₁ ≈ e₂): [Imp| <[var:id]> := <[arith:e₁]> ].equiv [Imp| <[var:id]> := <[arith:e₂]>] := by
       intro s₁ s₂
-      have h {id: String} {e₁ e₂: Arith} (h₁: e₁.equiv e₂): CommandEval (.assign id e₁) s₁ s₂ → CommandEval (.assign id e₂) s₁ s₂ := by
+      have h {id: String} {e₁ e₂: Arith} (h₁: e₁ ≈ e₂): (s₁ =[[Imp| <[var:id]> := <[arith:e₁]>]]=> s₂) → s₁ =[[Imp| <[var:id]> := <[arith:e₂]>]]=> s₂ := by
         intro
         | .assign _ h =>
           rw [h₁] at h
@@ -906,9 +926,9 @@ namespace SoftwareFoundations.ProgrammingLanguageFoundations.Equiv
       · apply h
         · exact Arith.equiv.symm h₁
 
-    theorem Command.seq.congr {c₁ c₂ c₃ c₄: Command} (h₁: c₁.equiv c₂) (h₂: c₃.equiv c₄): (Command.seq c₁ c₃).equiv (.seq c₂ c₄) := by
+    theorem Command.seq.congr {c₁ c₂ c₃ c₄: Command} (h₁: c₁ ≈ c₂) (h₂: c₃ ≈ c₄): [Imp| <[c₁]>; <[c₃]>] ≈ [Imp| <[c₂]>; <[c₄]>] := by
       intro s₁ s₂
-      have h {c₁ c₂ c₃ c₄: Command} (h₁: c₁.equiv c₂) (h₂: c₃.equiv c₄): CommandEval (.seq c₁ c₃) s₁ s₂ → CommandEval (.seq c₂ c₄) s₁ s₂ := by
+      have h {c₁ c₂ c₃ c₄: Command} (h₁: c₁ ≈ c₂) (h₂: c₃ ≈ c₄): (s₁ =[[Imp| <[c₁]>; <[c₃]>]]=> s₂) → s₁ =[[Imp| <[c₂]>; <[c₄]>]]=> s₂ := by
         intro
         | .seq _ _ _ h₃ h₄ =>
           rw [h₁] at h₃
@@ -920,9 +940,9 @@ namespace SoftwareFoundations.ProgrammingLanguageFoundations.Equiv
         · exact Command.equiv.symm h₁
         · exact Command.equiv.symm h₂
 
-    theorem Command.if.congr {c₁ c₂: Logic} {t₁ t₂ f₁ f₂: Command} (h₁: c₁.equiv c₂) (h₂: t₁.equiv t₂) (h₃: f₁.equiv f₂): (Command.if c₁ t₁ f₁).equiv (.if c₂ t₂ f₂) := by
+    theorem Command.if.congr {c₁ c₂: Logic} {t₁ t₂ f₁ f₂: Command} (h₁: c₁ ≈ c₂) (h₂: t₁ ≈ t₂) (h₃: f₁ ≈ f₂): [Imp| ite (<[expr:c₁]>) { <[t₁]> } else { <[f₁]> }] ≈ [Imp| ite (<[expr:c₂]>) { <[t₂]> } else { <[f₂]> }] := by
       intro s₁ s₂
-      have h {c₁ c₂: Logic} {t₁ t₂ f₁ f₂: Command} (h₁: c₁.equiv c₂) (h₂: t₁.equiv t₂) (h₃: f₁.equiv f₂): CommandEval (.if c₁ t₁ f₁) s₁ s₂ → CommandEval (.if c₂ t₂ f₂) s₁ s₂ := by
+      have h {c₁ c₂: Logic} {t₁ t₂ f₁ f₂: Command} (h₁: c₁ ≈ c₂) (h₂: t₁ ≈ t₂) (h₃: f₁ ≈ f₂): (s₁ =[[Imp| ite (<[expr:c₁]>) { <[t₁]> } else { <[f₁]> }]]=> s₂) → s₁ =[[Imp| ite (<[expr:c₂]>) { <[t₂]> } else { <[f₂]> }]]=> s₂ := by
         intro
         | .ifTrue _ _ h₄ h₅ =>
           rw [h₁] at h₄
@@ -939,14 +959,14 @@ namespace SoftwareFoundations.ProgrammingLanguageFoundations.Equiv
         · exact Command.equiv.symm h₂
         · exact Command.equiv.symm h₃
 
-    theorem Command.while.congr {c₁ c₂: Logic} {b₁ b₂: Command} (h₁: c₁.equiv c₂) (h₂: b₁.equiv b₂): (Command.while c₁ b₁).equiv (.while c₂ b₂) := by
+    theorem Command.while.congr {c₁ c₂: Logic} {b₁ b₂: Command} (h₁: c₁ ≈ c₂) (h₂: b₁ ≈ b₂): [Imp| while (<[expr:c₁]>) { <[b₁]> }] ≈ [Imp| while (<[expr:c₂]>) { <[b₂]> }] := by
       intro s₁ s₂
-      have h {c₁ c₂: Logic} {b₁ b₂: Command} (h₁: c₁.equiv c₂) (h₂: b₁.equiv b₂): CommandEval (.while c₁ b₁) s₁ s₂ → CommandEval (.while c₂ b₂) s₁ s₂ := by
+      have h {c₁ c₂: Logic} {b₁ b₂: Command} (h₁: c₁ ≈ c₂) (h₂: b₁ ≈ b₂): (s₁ =[[Imp| while (<[expr:c₁]>) { <[b₁]> }]]=> s₂) → s₁ =[[Imp| while (<[expr:c₂]>) { <[b₂]> }]]=> s₂ := by
         intro
         | .whileTrue s₃ s₄ s₅ h₃ h₄ h₅ =>
           rw [h₁] at h₃
           rw [h₂] at h₄
-          have ih: CommandEval (.while c₂ b₂) s₄ s₅ := by
+          have ih: s₄ =[[Imp| while (<[expr:c₂]>) { <[ b₂ ]>}]]=> s₅ := by
             sorry
           exact CommandEval.whileTrue _ _ _ h₃ h₄ ih
         | .whileFalse _ h₃ =>
@@ -962,21 +982,21 @@ namespace SoftwareFoundations.ProgrammingLanguageFoundations.Equiv
   end Tactic
 
   namespace Blended
-    theorem Command.skip.congr: Command.skip.equiv .skip
+    theorem Command.skip.congr: [Imp| skip] ≈ [Imp| skip]
       | _, _ => Iff.refl _
 
-    theorem Command.assign.congr {id: String} {e₁ e₂: Arith} (h₁: e₁.equiv e₂): (Command.assign id e₁).equiv (.assign id e₂)
+    theorem Command.assign.congr {id: String} {e₁ e₂: Arith} (h₁: e₁ ≈ e₂): [Imp| <[var:id]> := <[arith:e₁]> ].equiv [Imp| <[var:id]> := <[arith:e₂]>]
       | s₁, s₂ =>
-        have h {id: String} {e₁ e₂: Arith} (h₁: e₁.equiv e₂): CommandEval (.assign id e₁) s₁ s₂ → CommandEval (.assign id e₂) s₁ s₂
+        have h {id: String} {e₁ e₂: Arith} (h₁: e₁ ≈ e₂): (s₁ =[[Imp| <[var:id]> := <[arith:e₁]>]]=> s₂) → s₁ =[[Imp| <[var:id]> := <[arith:e₂]>]]=> s₂
           | .assign _ h => by
             rw [h₁] at h
             exact CommandEval.assign _ h
         have h₂ := Arith.equiv.symm h₁
         ⟨h h₁, h h₂⟩
 
-    theorem Command.seq.congr {c₁ c₂ c₃ c₄: Command} (h₁: c₁.equiv c₂) (h₂: c₃.equiv c₄): (Command.seq c₁ c₃).equiv (.seq c₂ c₄)
+    theorem Command.seq.congr {c₁ c₂ c₃ c₄: Command} (h₁: c₁ ≈ c₂) (h₂: c₃ ≈ c₄): [Imp| <[c₁]>; <[c₃]>] ≈ [Imp| <[c₂]>; <[c₄]>]
       | s₁, s₂ =>
-        have h {c₁ c₂ c₃ c₄: Command} (h₁: c₁.equiv c₂) (h₂: c₃.equiv c₄): CommandEval (.seq c₁ c₃) s₁ s₂ → CommandEval (.seq c₂ c₄) s₁ s₂
+        have h {c₁ c₂ c₃ c₄: Command} (h₁: c₁ ≈ c₂) (h₂: c₃ ≈ c₄): (s₁ =[[Imp| <[c₁]>; <[c₃]>]]=> s₂) → s₁ =[[Imp| <[c₂]>; <[c₄]>]]=> s₂
           | .seq _ _ _ h₃ h₄ => by
             rw [h₁] at h₃
             rw [h₂] at h₄
@@ -985,9 +1005,9 @@ namespace SoftwareFoundations.ProgrammingLanguageFoundations.Equiv
         have h₄ := Command.equiv.symm h₂
         ⟨h h₁ h₂, h h₃ h₄⟩
 
-    theorem Command.if.congr {c₁ c₂: Logic} {t₁ t₂ f₁ f₂: Command} (h₁: c₁.equiv c₂) (h₂: t₁.equiv t₂) (h₃: f₁.equiv f₂): (Command.if c₁ t₁ f₁).equiv (.if c₂ t₂ f₂)
+    theorem Command.if.congr {c₁ c₂: Logic} {t₁ t₂ f₁ f₂: Command} (h₁: c₁ ≈ c₂) (h₂: t₁ ≈ t₂) (h₃: f₁ ≈ f₂): [Imp| ite (<[expr:c₁]>) { <[t₁]> } else { <[f₁]> }] ≈ [Imp| ite (<[expr:c₂]>) { <[t₂]> } else { <[f₂]> }]
       | s₁, s₂ =>
-        have h {c₁ c₂: Logic} {t₁ t₂ f₁ f₂: Command} (h₁: c₁.equiv c₂) (h₂: t₁.equiv t₂) (h₃: f₁.equiv f₂): CommandEval (.if c₁ t₁ f₁) s₁ s₂ → CommandEval (.if c₂ t₂ f₂) s₁ s₂
+        have h {c₁ c₂: Logic} {t₁ t₂ f₁ f₂: Command} (h₁: c₁ ≈ c₂) (h₂: t₁ ≈ t₂) (h₃: f₁ ≈ f₂): (s₁ =[[Imp| ite (<[expr:c₁]>) { <[t₁]> } else { <[f₁]> }]]=> s₂) → s₁ =[[Imp| ite (<[expr:c₂]>) { <[t₂]> } else { <[f₂]> }]]=> s₂
           | .ifTrue _ _ h₄ h₅ => by
             rw [h₁] at h₄
             rw [h₂] at h₅
@@ -1001,9 +1021,9 @@ namespace SoftwareFoundations.ProgrammingLanguageFoundations.Equiv
         have h₆ := Command.equiv.symm h₃
         ⟨h h₁ h₂ h₃, h h₄ h₅ h₆⟩
 
-    theorem Command.while.congr {c₁ c₂: Logic} {b₁ b₂: Command} (h₁: c₁.equiv c₂) (h₂: b₁.equiv b₂): (Command.while c₁ b₁).equiv (.while c₂ b₂)
+    theorem Command.while.congr {c₁ c₂: Logic} {b₁ b₂: Command} (h₁: c₁ ≈ c₂) (h₂: b₁ ≈ b₂): [Imp| while (<[expr:c₁]>) { <[b₁]> }] ≈ [Imp| while (<[expr:c₂]>) { <[b₂]> }]
       | s₁, s₂ =>
-        have h {c₁ c₂: Logic} {b₁ b₂: Command} (h₁: c₁.equiv c₂) (h₂: b₁.equiv b₂): CommandEval (.while c₁ b₁) s₁ s₂ → CommandEval (.while c₂ b₂) s₁ s₂
+        have h {c₁ c₂: Logic} {b₁ b₂: Command} (h₁: c₁ ≈ c₂) (h₂: b₁ ≈ b₂): (s₁ =[[Imp| while (<[expr:c₁]>) { <[b₁]> }]]=> s₂) → s₁ =[[Imp| while (<[expr:c₂]>) { <[b₂]> }]]=> s₂
           | .whileTrue s₃ s₄ s₅ h₃ h₄ h₅ => by
             rw [h₁] at h₃
             rw [h₂] at h₄
@@ -1027,9 +1047,9 @@ namespace SoftwareFoundations.ProgrammingLanguageFoundations.Equiv
   ## Program Transformations
   -/
 
-  def Arith.transform_sound (t: Arith → Arith): Prop := ∀ e: Arith, e.equiv (t e)
-  def Logic.transform_sound (t: Logic → Logic): Prop := ∀ b: Logic, b.equiv (t b)
-  def Command.transform_sound (t: Command → Command): Prop := ∀ c: Command, c.equiv (t c)
+  def Arith.transform_sound (t: Arith → Arith): Prop := ∀ e: Arith, e ≈ (t e)
+  def Logic.transform_sound (t: Logic → Logic): Prop := ∀ b: Logic, b ≈ (t b)
+  def Command.transform_sound (t: Command → Command): Prop := ∀ c: Command, c ≈ (t c)
 
   /-
   ### Constant Folding Optimization
@@ -1052,8 +1072,8 @@ namespace SoftwareFoundations.ProgrammingLanguageFoundations.Equiv
         | .num n₁, .num n₂ => .num (n₁ * n₂)
         | e₁, e₂ => .mult e₁ e₂
 
-  example: (((1: Arith) + 2) * "X").constFold = 3 * "X" := rfl
-  example: ("X" - (((0: Arith) * 6) + "Y")).constFold = "X" - (0 + "Y") := rfl
+  example: [Arith| (1 + 2) * X].constFold = [Arith|3 * X] := rfl
+  example: [Arith| X - ((0 * 6) + Y)].constFold = [Arith| X - (0 + Y)] := rfl
 
   @[reducible]
   def _root_.SoftwareFoundations.LogicalFoundations.Imp.Logic.constFold: Logic → Logic
@@ -1090,8 +1110,8 @@ namespace SoftwareFoundations.ProgrammingLanguageFoundations.Equiv
         | .false, .false => .false
         | b₁, b₂ => .and b₁ b₂
 
-  example: (Logic.and .true (.not (.false && .true))).constFold = .true := rfl
-  example: (Logic.and (.eq "X" "Y") (.eq 0 (2 - (1 + 1)))).constFold = .and (.eq "X" "Y") .true := rfl
+  example: [Logic| tru && !(fls && tru)].constFold = [Logic| tru] := rfl
+  example: [Logic| (X = Y) && (0 = (2 - (1 + 1)))].constFold = [Logic| (X = Y) && tru] := rfl
 
   @[reducible]
   def _root_.SoftwareFoundations.LogicalFoundations.Imp.Command.constFold: Command → Command
@@ -1112,33 +1132,37 @@ namespace SoftwareFoundations.ProgrammingLanguageFoundations.Equiv
         | c => .while c b.constFold
 
   example:
-    (Command.seq
-      (.assign "X" (4 + 5))
-      (Command.seq
-        (.assign "Y" ("X" - 3))
-        (Command.seq
-          (.if (.eq ("X" - "Y") (2 + 4))
-            .skip
-            (.assign "Y" 0))
-          (Command.seq
-            (.if (.le 0 (4 - (2 + 1)))
-              (.assign "Y" 0)
-              .skip)
-            (.while (.eq "Y" 0)
-              (.assign "X" ("X" + 1))))))).constFold
+    [Imp|
+      X := 4 + 5;
+      Y := X - 3;
+      ite ((X - Y) = (2 + 4)) {
+        skip
+      } else {
+        Y := 0
+      };
+      ite (0 ≤ (4 - (2 + 1))) {
+        Y := 0
+      } else {
+        skip
+      };
+      while (Y = 0) {
+        X := X + 1
+      }
+    ].constFold
     =
-    Command.seq
-    (.assign "X" 9)
-    (Command.seq
-      (.assign "Y" ("X" - 3))
-      (Command.seq
-        (.if (.eq ("X" - "Y") 6)
-          .skip
-          (.assign "Y" 0))
-        (Command.seq
-          (.assign "Y" 0)
-          (.while (.eq "Y" 0)
-            (.assign "X" ("X" + 1))))))
+    [Imp|
+      X := 9;
+      Y := X - 3;
+      ite ((X - Y) = 6) {
+        skip
+      } else {
+        Y := 0
+      };
+      Y := 0;
+      while (Y = 0) {
+        X := X + 1
+      }
+    ]
     := rfl
 
   /-
@@ -1170,21 +1194,21 @@ namespace SoftwareFoundations.ProgrammingLanguageFoundations.Equiv
         have ih₁ := sound e₁ s
         have ih₂ := sound e₂ s
         have h :=
-          calc (Arith.minus e₁ e₂).eval s
-            _ = e₁.eval s - e₂.eval s                          := rfl
-            _ = e₁.constFold.eval s - e₂.constFold.eval s      := congr (congrArg Nat.sub ih₁) ih₂
-            _ = (Arith.minus e₁.constFold e₂.constFold).eval s := rfl
-            -- _ = (Arith.minus e₁ e₂).constFold.eval s           := sorry
+          calc [Arith| <[expr:e₁]> - <[expr:e₂]>].eval s
+            _ = e₁.eval s - e₂.eval s                                         := rfl
+            _ = e₁.constFold.eval s - e₂.constFold.eval s                     := congr (congrArg Nat.sub ih₁) ih₂
+            _ = [Arith| <[expr:e₁.constFold]> - <[expr:e₂.constFold]>].eval s := rfl
+            -- _ = [Arith| <[expr:e₁]> - <[expr:e₂]>].eval s                     := sorry
         sorry
       | .mult e₁ e₂, s =>
         have ih₁ := sound e₁ s
         have ih₂ := sound e₂ s
         have h :=
-          calc (Arith.mult e₁ e₂).eval s
-            _ = e₁.eval s * e₂.eval s                         := rfl
-            _ = e₁.constFold.eval s * e₂.constFold.eval s     := congr (congrArg Nat.mul ih₁) ih₂
-            _ = (Arith.mult e₁.constFold e₂.constFold).eval s := rfl
-            -- _ = (Arith.mult e₁ e₂).constFold.eval s           := sorry
+          calc [Arith| <[expr:e₁]> * <[expr:e₂]>].eval s
+            _ = e₁.eval s * e₂.eval s                                         := rfl
+            _ = e₁.constFold.eval s * e₂.constFold.eval s                     := congr (congrArg Nat.mul ih₁) ih₂
+            _ = [Arith| <[expr:e₁.constFold]> * <[expr:e₂.constFold]>].eval s := rfl
+            -- _ = [Arith| <[expr:e₁]> * <[expr:e₂]>].eval s                     := sorry
         sorry
 
     theorem Logic.constFold.sound: Logic.transform_sound Logic.constFold := sorry
@@ -1253,7 +1277,7 @@ namespace SoftwareFoundations.ProgrammingLanguageFoundations.Equiv
     | .while c b => .while c.opt0Plus (opt0Plus b)
     | c => c
 
-  example: (Command.while (.neq "X" 0) (.assign "X" (0 + "X" - 1))).opt0Plus = .while (.neq "X" 0) (.assign "X" ("X" - 1)) := rfl
+  example: [Imp| while (X ≠ 0) { X := 0 + X - 1 }].opt0Plus = [Imp| while (X ≠ 0) { X := X - 1 }] := rfl
 
   namespace Term
     theorem Arith.opt0Plus.sound: Arith.transform_sound Arith.opt0Plus
@@ -1265,97 +1289,97 @@ namespace SoftwareFoundations.ProgrammingLanguageFoundations.Equiv
           | .num n =>
             match n with
               | .zero =>
-                calc (Arith.plus (.num 0) e₂).eval s
-                  _ = (Arith.num 0).eval s + e₂.eval s                       := rfl
-                  _ = (Arith.num 0).opt0Plus.eval s + e₂.opt0Plus.eval s     := congr (congrArg Nat.add ih₁) ih₂
-                  _ = (Arith.plus (Arith.num 0).opt0Plus e₂.opt0Plus).eval s := rfl
-                  _ = (Arith.plus (Arith.num 0) e₂).opt0Plus.eval s          := by simp -- congrArg (Arith.eval s) rfl -- TODO: Remove Tactic Block
-                  _ = e₂.opt0Plus.eval s                                     := rfl
+                calc [Arith| 0 + <[expr:e₂]>].eval s
+                  _ = [Arith| 0].eval s + e₂.eval s                                       := rfl
+                  _ = [Arith| 0].opt0Plus.eval s + e₂.opt0Plus.eval s                     := congr (congrArg Nat.add ih₁) ih₂
+                  _ = [Arith| <[expr:[Arith| 0].opt0Plus]> + <[expr:e₂.opt0Plus]>].eval s := rfl
+                  _ = [Arith| 0 + <[expr:e₂]>].opt0Plus.eval s                            := by simp -- congrArg (Arith.eval s) rfl -- TODO: Remove Tactic Block
+                  _ = e₂.opt0Plus.eval s                                                  := rfl
               | .succ _ =>
-                calc (Arith.plus (.num (.succ _)) e₂).eval s
+                calc [Arith| <[num:Nat.succ _]> + <[expr:e₂]>].eval s
                   _ = (Arith.num (.succ _)).eval s + e₂.eval s                   := rfl
                   _ = (Arith.num (.succ _)).opt0Plus.eval s + e₂.opt0Plus.eval s := congr (congrArg Nat.add ih₁) ih₂
                   _ = (Arith.plus (.num (.succ _)) e₂).opt0Plus.eval s           := rfl
           | .ident _ =>
-            calc (Arith.plus (.ident _) e₂).eval s
-              _ = (Arith.ident _).eval s + e₂.eval s                   := rfl
-              _ = (Arith.ident _).opt0Plus.eval s + e₂.opt0Plus.eval s := congr (congrArg Nat.add ih₁) ih₂
-              _ = (Arith.plus (.ident _) e₂).opt0Plus.eval s           := rfl
+            calc [Arith| <[id:_]> + <[expr:e₂]>].eval s
+              _ = [Arith| <[id:_]>].eval s + e₂.eval s                   := rfl
+              _ = [Arith| <[id:_]>].opt0Plus.eval s + e₂.opt0Plus.eval s := congr (congrArg Nat.add ih₁) ih₂
+              _ = [Arith| <[id:_]> + <[expr:e₂]>].opt0Plus.eval s        := rfl
           | .plus _ _ =>
-            calc (Arith.plus (.plus _ _) e₂).eval s
-              _ = (Arith.plus _ _).eval s + e₂.eval s                   := rfl
-              _ = (Arith.plus _ _).opt0Plus.eval s + e₂.opt0Plus.eval s := congr (congrArg Nat.add ih₁) ih₂
-              _ = (Arith.plus (.plus _ _) e₂).opt0Plus.eval s           := rfl
+            calc [Arith| (<[expr:_]> + <[expr:_]>) + <[expr:e₂]>].eval s
+              _ = [Arith| <[expr:_]> + <[expr:_]>].eval s + e₂.eval s                   := rfl
+              _ = [Arith| <[expr:_]> + <[expr:_]>].opt0Plus.eval s + e₂.opt0Plus.eval s := congr (congrArg Nat.add ih₁) ih₂
+              _ = [Arith| (<[expr:_]> + <[expr:_]>) + <[expr:e₂]>].opt0Plus.eval s      := rfl
           | .minus _ _ =>
-            calc (Arith.plus (.minus _ _) e₂).eval s
-              _ = (Arith.minus _ _).eval s + e₂.eval s                   := rfl
-              _ = (Arith.minus _ _).opt0Plus.eval s + e₂.opt0Plus.eval s := congr (congrArg Nat.add ih₁) ih₂
-              _ = (Arith.plus (.minus _ _) e₂).opt0Plus.eval s           := rfl
+            calc [Arith| (<[expr:_]> - <[expr:_]>) + <[expr:e₂]>].eval s
+              _ = [Arith| <[expr:_]> - <[expr:_]>].eval s + e₂.eval s                   := rfl
+              _ = [Arith| <[expr:_]> - <[expr:_]>].opt0Plus.eval s + e₂.opt0Plus.eval s := congr (congrArg Nat.add ih₁) ih₂
+              _ = [Arith| (<[expr:_]> - <[expr:_]>) + <[expr:e₂]>].opt0Plus.eval s      := rfl
           | .mult _ _ =>
-            calc (Arith.plus (.mult _ _) e₂).eval s
-              _ = (Arith.mult _ _).eval s + e₂.eval s                   := rfl
-              _ = (Arith.mult _ _).opt0Plus.eval s + e₂.opt0Plus.eval s := congr (congrArg Nat.add ih₁) ih₂
-              _ = (Arith.plus (.mult _ _) e₂).opt0Plus.eval s           := rfl
+            calc [Arith| (<[expr:_]> * <[expr:_]>) + <[expr:e₂]>].eval s
+              _ = [Arith| <[expr:_]> * <[expr:_]>].eval s + e₂.eval s                   := rfl
+              _ = [Arith| <[expr:_]> * <[expr:_]>].opt0Plus.eval s + e₂.opt0Plus.eval s := congr (congrArg Nat.add ih₁) ih₂
+              _ = [Arith| (<[expr:_]> * <[expr:_]>) + <[expr:e₂]>].opt0Plus.eval s      := rfl
       | .minus e₁ e₂, s =>
         have ih₁ := sound e₁ s
         have ih₂ := sound e₂ s
-        calc (Arith.minus e₁ e₂).eval s
-          _ = e₁.eval s - e₂.eval s                   := rfl
-          _ = e₁.opt0Plus.eval s - e₂.opt0Plus.eval s := congr (congrArg Nat.sub ih₁) ih₂
-          _ = (Arith.minus e₁ e₂).opt0Plus.eval s     := rfl
+        calc [Arith| <[expr:e₁]> - <[expr:e₂]>].eval s
+          _ = e₁.eval s - e₂.eval s                              := rfl
+          _ = e₁.opt0Plus.eval s - e₂.opt0Plus.eval s            := congr (congrArg Nat.sub ih₁) ih₂
+          _ = [Arith| <[expr:e₁]> - <[expr:e₂]>].opt0Plus.eval s := rfl
       | .mult e₁ e₂, s =>
         have ih₁ := sound e₁ s
         have ih₂ := sound e₂ s
-        calc (Arith.mult e₁ e₂).eval s
-          _ = e₁.eval s * e₂.eval s                   := rfl
-          _ = e₁.opt0Plus.eval s * e₂.opt0Plus.eval s := congr (congrArg Nat.mul ih₁) ih₂
-          _ = (Arith.mult e₁ e₂).opt0Plus.eval s      := rfl
+        calc [Arith| <[expr:e₁]> * <[expr:e₂]>].eval s
+          _ = e₁.eval s * e₂.eval s                              := rfl
+          _ = e₁.opt0Plus.eval s * e₂.opt0Plus.eval s            := congr (congrArg Nat.mul ih₁) ih₂
+          _ = [Arith| <[expr:e₁]> * <[expr:e₂]>].opt0Plus.eval s := rfl
 
     theorem Logic.opt0Plus.sound: Logic.transform_sound Logic.opt0Plus
       | .true, _ | .false, _ => rfl
       | .eq e₁ e₂, s =>
         have ih₁ := Arith.opt0Plus.sound e₁ s
         have ih₂ := Arith.opt0Plus.sound e₂ s
-        calc (Logic.eq e₁ e₂).eval s
+        calc [Logic| <[expr:e₁]> = <[expr:e₂]>].eval s
           _ = BEq.beq (e₁.eval s) (e₂.eval s)                   := rfl
           _ = BEq.beq (e₁.opt0Plus.eval s) (e₂.opt0Plus.eval s) := congr (congrArg BEq.beq ih₁) ih₂
-          _ = (Logic.eq e₁ e₂).opt0Plus.eval s                  := rfl
+          _ = [Logic| <[expr:e₁]> = <[expr:e₂]>].opt0Plus.eval s                  := rfl
       | .neq e₁ e₂, s =>
         have ih₁ := Arith.opt0Plus.sound e₁ s
         have ih₂ := Arith.opt0Plus.sound e₂ s
-        calc (Logic.neq e₁ e₂).eval s
+        calc [Logic| <[expr:e₁]> ≠ <[expr:e₂]>].eval s
           _ = not (BEq.beq (e₁.eval s) (e₂.eval s))                   := rfl
           _ = not (BEq.beq (e₁.opt0Plus.eval s) (e₂.opt0Plus.eval s)) := sorry-- congr (congr (congrArg (not ∘ BEq.beq)) ih₁) ih₂
-          _ = (Logic.neq e₁ e₂).opt0Plus.eval s                       := rfl
+          _ = [Logic| <[expr:e₁]> ≠ <[expr:e₂]>].opt0Plus.eval s                       := rfl
       | .le e₁ e₂, s =>
         have ih₁ := Arith.opt0Plus.sound e₁ s
         have ih₂ := Arith.opt0Plus.sound e₂ s
         sorry
-        -- calc (Logic.le e₁ e₂).eval s
+        -- calc [Logic| <[expr:e₁]> ≤ <[expr:e₂]>].eval s
         --   _ = (LE.le (e₁.eval s) (e₂.eval s): Bool)                   := rfl
         --   _ = (LE.le (e₁.opt0Plus.eval s) (e₂.opt0Plus.eval s): Bool) := congr (congrArg LE.le ih₁) ih₂
-        --   _ = (Logic.le e₁ e₂).opt0Plus.eval s                        := rfl
+        --   _ = [Logic| <[expr:e₁]> ≤ <[expr:e₂]>].opt0Plus.eval s                        := rfl
       | .gt e₁ e₂, s =>
         have ih₁ := Arith.opt0Plus.sound e₁ s
         have ih₂ := Arith.opt0Plus.sound e₂ s
         sorry
-        -- calc (Logic.gt e₁ e₂).eval s
+        -- calc [Logic| <[expr:e₁]> > <[expr:e₂]>].eval s
         --   _ = (GT.gt (e₁.eval s) (e₂.eval s): Bool)                   := rfl
         --   _ = (GT.gt (e₁.opt0Plus.eval s) (e₂.opt0Plus.eval s): Bool) := congr (congrArg GT.gt ih₁) ih₂
-        --   _ = (Logic.gt e₁ e₂).opt0Plus.eval s                        := rfl
+        --   _ = [Logic| <[expr:e₁]> > <[expr:e₂]>].opt0Plus.eval s                        := rfl
       | .not b, s =>
         have ih := sound b s
-        calc (Logic.not b).eval s
+        calc [Logic| ! <[expr:b]>].eval s
           _ = not (b.eval s)                := rfl
           _ = not (b.opt0Plus.eval s)       := congrArg not ih
-          _ = (Logic.not b).opt0Plus.eval s := rfl
+          _ = [Logic| ! <[expr:b]> ].opt0Plus.eval s := rfl
       | .and b₁ b₂, s =>
         have ih₁ := sound b₁ s
         have ih₂ := sound b₂ s
-        calc (Logic.and b₁ b₂).eval s
+        calc [Logic| <[expr:b₁]> && <[expr:b₂]> ].eval s
           _ = and (b₁.eval s) (b₂.eval s)                   := rfl
           _ = and (b₁.opt0Plus.eval s) (b₂.opt0Plus.eval s) := congr (congrArg and ih₁) ih₂
-          _ = (Logic.and b₁ b₂).opt0Plus.eval s             := rfl
+          _ = [Logic| <[expr:b₁]> && <[expr:b₂]> ].opt0Plus.eval s             := rfl
 
     theorem Command.opt0Plus.sound: Command.transform_sound Command.opt0Plus
       | .skip, _, _ => ⟨id, id⟩
@@ -1379,25 +1403,26 @@ namespace SoftwareFoundations.ProgrammingLanguageFoundations.Equiv
 
   namespace Tactic
     theorem Arith.opt0Plus.sound: Arith.transform_sound Arith.opt0Plus := by
-      intro e s
-      induction e
-      <;> try rfl
-      case minus | mult =>
-        unfold Arith.opt0Plus Arith.eval
-        simp_all
-      case plus e₁ e₂ ih₁ ih₂ =>
-        cases e₁
-        case num n =>
-          cases n with
-            | zero =>
-              repeat rw [← ih₂]
-              simp_all
-            | succ n =>
-              unfold Arith.opt0Plus
-              simp_all
-        case ident | plus | minus | mult =>
-          unfold Arith.opt0Plus Arith.eval
-          simp_all
+      -- intro e s
+      -- induction e
+      -- <;> try rfl
+      -- case minus | mult =>
+      --   unfold Arith.opt0Plus Arith.eval
+      --   simp_all
+      -- case plus e₁ e₂ ih₁ ih₂ =>
+      --   cases e₁
+      --   case num n =>
+      --     cases n with
+      --       | zero =>
+      --         repeat rw [← ih₂]
+      --         simp_all
+      --       | succ n =>
+      --         unfold Arith.opt0Plus
+      --         simp_all
+      --   case ident | plus | minus | mult =>
+      --     unfold Arith.opt0Plus Arith.eval
+      --     simp_all
+       sorry
 
     theorem Logic.opt0Plus.sound: Logic.transform_sound Logic.opt0Plus := by
       intro b s
@@ -1424,10 +1449,10 @@ namespace SoftwareFoundations.ProgrammingLanguageFoundations.Equiv
             match n with
               | .zero => by simp_all
               | .succ _ =>
-                calc (Arith.plus (Arith.num (.succ _)) e₂).eval s
+                calc [Arith| <[num:Nat.succ _]> + <[expr:e₂]>].eval s
                   _ = (Arith.num (.succ _)).eval s + e₂.eval s                   := by rfl
                   _ = (Arith.num (.succ _)).opt0Plus.eval s + e₂.opt0Plus.eval s := by rw [ih₁, ih₂]
-                  _ = (Arith.plus (Arith.num (.succ _)) e₂).opt0Plus.eval s      := by rfl
+                  _ = (Arith.plus (.num (.succ _)) e₂).opt0Plus.eval s           := by rfl
           | .ident _ | .plus _ _ | .minus _ _ | .mult _ _ =>
             by
               unfold Arith.eval
@@ -1459,7 +1484,24 @@ namespace SoftwareFoundations.ProgrammingLanguageFoundations.Equiv
           unfold Logic.eval
           rw [ih₁, ih₂]
 
-    theorem Command.opt0Plus.sound: Command.transform_sound Command.opt0Plus := sorry
+    theorem Command.opt0Plus.sound: Command.transform_sound Command.opt0Plus
+      | .skip, _, _ => ⟨id, id⟩
+      | .assign _ e, s₁, s₂ =>
+        have h := Arith.opt0Plus.sound e
+        Command.assign.congr h s₁ s₂
+      | .seq c₁ c₂, s₁, s₂ =>
+        have h₁ := sound c₁
+        have h₂ := sound c₂
+        Command.seq.congr h₁ h₂ s₁ s₂
+      | .if c t f, s₁, s₂ =>
+        have h₁ := Logic.opt0Plus.sound c
+        have h₂ := sound t
+        have h₃ := sound f
+        Command.if.congr h₁ h₂ h₃ s₁ s₂
+      | .while c b, s₁, s₂ =>
+        have h₁ := Logic.opt0Plus.sound c
+        have h₂ := sound b
+        Command.while.congr h₁ h₂ s₁ s₂
   end Blended
 
   /-
@@ -1494,9 +1536,9 @@ namespace SoftwareFoundations.ProgrammingLanguageFoundations.Equiv
       | .minus e₁ e₂ => .minus (subst e₁ var repl) (subst e₂ var repl)
       | .mult e₁ e₂ => .mult (subst e₁ var repl) (subst e₂ var repl)
 
-  example: (("Y": Arith) + "X").subst "X" (42 + 53) = "Y" + (42 + 53) := rfl
+  example: [Arith| Y + X].subst "X" [Arith|42 + 53] = [Arith| Y + (42 + 53)] := rfl
 
-  def Arith.subst.equiv: Prop := ∀ id₁ id₂ e₁ e₂, (Command.seq (.assign id₁ e₁) (.assign id₂ e₂)).equiv (.seq (.assign id₁ e₁) (.assign id₂ (e₂.subst id₁ e₁)))
+  def Arith.subst.equiv: Prop := ∀ id₁ id₂ e₁ e₂, [Imp| <[var:id₁]> := <[arith:e₁]>; <[var:id₂]> := <[arith:e₂]>] ≈ [Imp| <[var:id₁]> := <[arith:e₁]>; <[var:id₂]> := <[arith:e₂.subst id₁ e₁]>]
 
   namespace Term
     theorem Arith.subst.equiv.inequiv: ¬Arith.subst.equiv := sorry
@@ -1557,70 +1599,72 @@ namespace SoftwareFoundations.ProgrammingLanguageFoundations.Equiv
 
     def Command.equiv (c₁ c₂: Command): Prop := ∀ s₁ s₂: State, CommandEval c₁ s₁ s₂ ↔ CommandEval c₂ s₁ s₂
 
+    infix:50 "≈" => Command.equiv
+
     private def xy: Command := .seq (.havoc "X") (.havoc "Y")
     private def yx: Command := .seq (.havoc "Y") (.havoc "X")
-    private def copy: Command := .seq (.havoc "X") (.assign "Y" "X")
+    private def copy: Command := .seq (.havoc "X") (.assign "Y" [Arith| X])
     private def whileHavoc: Command :=
-      .while (.not (.eq "X" 0))
-        (.seq (.havoc "X") (.assign "X" ("X" + 1)))
-    private def whileSkip: Command := .while (.not (.eq "X" 0)) .skip
+      .while [Logic| !(X = 0)]
+        (.seq (.havoc "X") (.assign "X" [Arith| X + 1]))
+    private def whileSkip: Command := .while [Logic| !(X = 0)] .skip
     private def havocHavoc: Command :=
-      .while (.neq "X" 0)
+      .while [Logic| X ≠ 0]
         (.seq (.havoc "X") (.havoc "Y"))
-    private def noHavoc: Command := .seq (.assign "X" 0) (.assign "Z" 1)
+    private def noHavoc: Command := .seq (.assign "X" [Arith| 0]) (.assign "Z" [Arith| 1])
 
     namespace Term
-      example: CommandEval (.havoc "X") State.empty (State.build [("X", 0)]) := sorry
-      example: CommandEval (.seq .skip (.havoc "Z")) State.empty (State.build [("Z", 42)]) := sorry
+      example: CommandEval (.havoc "X") [State|] [State| X = 0] := sorry
+      example: CommandEval (.seq .skip (.havoc "Z")) [State|] [State| Z = 42] := sorry
 
-      example: xy.equiv yx ∨ ¬(xy.equiv yx) := sorry
-      example: xy.equiv copy ∨ ¬(xy.equiv copy) := sorry
+      example: xy ≈ yx ∨ ¬(xy ≈ yx) := sorry
+      example: xy ≈ copy ∨ ¬(xy ≈ copy) := sorry
 
-      example: whileHavoc.equiv whileSkip :=
+      example: whileHavoc ≈ whileSkip :=
         sorry
         where
           havoc_may_diverge (s₁ s₂: State) (h: s₁ "X" ≠ 0): ¬(CommandEval whileHavoc s₁ s₂) := sorry
           skip_may_diverge (s₁ s₂: State) (h: s₁ "X" ≠ 0): ¬(CommandEval whileSkip s₁ s₂) := sorry
 
-      example: ¬(havocHavoc.equiv noHavoc) := sorry
+      example: ¬(havocHavoc ≈ noHavoc) := sorry
 
-      example: (Command.while (.neq "X" 1) (.havoc "X")).equiv (.assign "X" 1) := sorry
+      example: (Command.while [Logic| X ≠ 1] (.havoc "X")) ≈ (.assign "X" [Arith|1]) := sorry
     end Term
 
     namespace Tactic
-      example: CommandEval (.havoc "X") State.empty (State.build [("X", 0)]) := by sorry
-      example: CommandEval (.seq .skip (.havoc "Z")) State.empty (State.build [("Z", 42)]) := by sorry
+      example: CommandEval (.havoc "X") [State|] [State| X = 0] := by sorry
+      example: CommandEval (.seq .skip (.havoc "Z")) [State|] [State| Z = 42] := by sorry
 
-      example: xy.equiv yx ∨ ¬(xy.equiv yx) := by sorry
-      example: xy.equiv copy ∨ ¬(xy.equiv copy) := by sorry
+      example: xy ≈ yx ∨ ¬(xy ≈ yx) := by sorry
+      example: xy ≈ copy ∨ ¬(xy ≈ copy) := by sorry
 
-      example: whileHavoc.equiv whileSkip := by
+      example: whileHavoc ≈ whileSkip := by
         sorry
         where
           havoc_may_diverge (s₁ s₂: State) (h: s₁ "X" ≠ 0): ¬(CommandEval whileHavoc s₁ s₂) := by sorry
           skip_may_diverge (s₁ s₂: State) (h: s₁ "X" ≠ 0): ¬(CommandEval whileSkip s₁ s₂) := by sorry
 
-      example: ¬(havocHavoc.equiv noHavoc) := by sorry
+      example: ¬(havocHavoc ≈ noHavoc) := by sorry
 
-      example: (Command.while (.neq "X" 1) (.havoc "X")).equiv (.assign "X" 1) := by sorry
+      example: (Command.while [Logic| X ≠ 1] (.havoc "X")) ≈ (.assign "X" [Arith|1]) := sorry
     end Tactic
 
     namespace Blended
-      example: CommandEval (.havoc "X") State.empty (State.build [("X", 0)]) := sorry
-      example: CommandEval (.seq .skip (.havoc "Z")) State.empty (State.build [("Z", 42)]) := sorry
+      example: CommandEval (.havoc "X") [State|] [State| X = 0] := sorry
+      example: CommandEval (.seq .skip (.havoc "Z")) [State|] [State| Z = 42] := sorry
 
-      example: xy.equiv yx ∨ ¬(xy.equiv yx) := sorry
-      example: xy.equiv copy ∨ ¬(xy.equiv copy) := sorry
+      example: xy ≈ yx ∨ ¬(xy ≈ yx) := sorry
+      example: xy ≈ copy ∨ ¬(xy ≈ copy) := sorry
 
-      example: whileHavoc.equiv whileSkip :=
+      example: whileHavoc ≈ whileSkip :=
         sorry
         where
           havoc_may_diverge (s₁ s₂: State) (h: s₁ "X" ≠ 0): ¬(CommandEval whileHavoc s₁ s₂) := sorry
           skip_may_diverge (s₁ s₂: State) (h: s₁ "X" ≠ 0): ¬(CommandEval whileSkip s₁ s₂) := sorry
 
-      example: ¬(havocHavoc.equiv noHavoc) := sorry
+      example: ¬(havocHavoc ≈ noHavoc) := sorry
 
-      example: (Command.while (.neq "X" 1) (.havoc "X")).equiv (.assign "X" 1) := sorry
+      example: (Command.while [Logic| X ≠ 1] (.havoc "X")) ≈ (.assign "X" [Arith|1]) := sorry
     end Blended
   end Havoc
 
@@ -1629,10 +1673,10 @@ namespace SoftwareFoundations.ProgrammingLanguageFoundations.Equiv
   -/
 
   -- How is this different from "refines" above?
-  @[reducible] def _root_.SoftwareFoundations.LogicalFoundations.Imp.Command.approx  (c₁ c₂: Command): Prop := ∀ s₁ s₂: State, CommandEval c₁ s₁ s₂ → CommandEval c₂ s₁ s₂
+  @[reducible] def _root_.SoftwareFoundations.LogicalFoundations.Imp.Command.approx  (c₁ c₂: Command): Prop := ∀ s₁ s₂: State, (s₁ =[c₁]=> s₂) → s₁ =[c₂]=> s₂
 
-  private def approx_c₁: Command := .while (.neq "X" 1) (.assign "X" ("X" - 1))
-  private def approx_c₂: Command := .assign "X" 1
+  private def approx_c₁ := [Imp| while (X ≠ 1) { X := X - 1}]
+  private def approx_c₂ := [Imp| X := 1]
 
   private def approx_c₃: Command := sorry
   private def approx_c₄: Command := sorry
@@ -1642,7 +1686,7 @@ namespace SoftwareFoundations.ProgrammingLanguageFoundations.Equiv
   private def _root_.SoftwareFoundations.LogicalFoundations.Imp.Command.zProp (c: Command): Prop := sorry
 
   namespace Term
-    example (id₁ id₂: String) (e₁ e₂: Arith) (h₁: OccursCheck id₁ e₁) (h₂: OccursCheck id₂ e₂): (Command.seq (.assign id₁ e₁) (.assign id₂ e₂)).equiv (.seq (.assign id₂ e₂) (.assign id₁ e₁)) := sorry
+    example (id₁ id₂: String) (e₁ e₂: Arith) (h₁: OccursCheck id₁ e₁) (h₂: OccursCheck id₂ e₂): [Imp| <[var:id₁]> := <[arith:e₁]>; <[var:id₂]> := <[arith:e₂]>] ≈ [Imp| <[var:id₂]> := <[arith:e₂]>; <[var:id₁]> := <[arith:e₁]>] := sorry
 
     -- TODO: For loops in Imp
 
@@ -1652,7 +1696,7 @@ namespace SoftwareFoundations.ProgrammingLanguageFoundations.Equiv
   end Term
 
   namespace Tactic
-    example (id₁ id₂: String) (e₁ e₂: Arith) (h₁: OccursCheck id₁ e₁) (h₂: OccursCheck id₂ e₂): (Command.seq (.assign id₁ e₁) (.assign id₂ e₂)).equiv (.seq (.assign id₂ e₂) (.assign id₁ e₁)) := by sorry
+    example (id₁ id₂: String) (e₁ e₂: Arith) (h₁: OccursCheck id₁ e₁) (h₂: OccursCheck id₂ e₂): [Imp| <[var:id₁]> := <[arith:e₁]>; <[var:id₂]> := <[arith:e₂]>] ≈ [Imp| <[var:id₂]> := <[arith:e₂]>; <[var:id₁]> := <[arith:e₁]>] := by sorry
 
     -- TODO: For loops in Imp
 
@@ -1662,7 +1706,7 @@ namespace SoftwareFoundations.ProgrammingLanguageFoundations.Equiv
   end Tactic
 
   namespace Blended
-    example (id₁ id₂: String) (e₁ e₂: Arith) (h₁: OccursCheck id₁ e₁) (h₂: OccursCheck id₂ e₂): (Command.seq (.assign id₁ e₁) (.assign id₂ e₂)).equiv (.seq (.assign id₂ e₂) (.assign id₁ e₁)) := sorry
+    example (id₁ id₂: String) (e₁ e₂: Arith) (h₁: OccursCheck id₁ e₁) (h₂: OccursCheck id₂ e₂): [Imp| <[var:id₁]> := <[arith:e₁]>; <[var:id₂]> := <[arith:e₂]>] ≈ [Imp| <[var:id₂]> := <[arith:e₂]>; <[var:id₁]> := <[arith:e₁]>] := sorry
 
     -- TODO: For loops in Imp
 
