SoftwareFoundations/ProgrammingLanguageFoundations/Hoare.lean
@@ -13,6 +13,8 @@ namespace SoftwareFoundations.ProgrammingLanguageFoundations.Hoare
   -/
 
   def Assertion: Type := State → Prop
+  def NatAssertion: Type := State → Nat
+  def ArithAssertion: Type := State → Arith
 
   section
     private def assertionOne: Assertion
@@ -25,19 +27,65 @@ namespace SoftwareFoundations.ProgrammingLanguageFoundations.Hoare
       | s => s "Z" = max (s "X") (s "Y")
   end
 
+  instance: Coe Nat NatAssertion where
+    coe n := fun _ => n
+  instance: Coe String NatAssertion where
+    coe id := fun s => s id
+  instance: OfNat NatAssertion n where
+    ofNat := (n: NatAssertion)
+  instance: Coe Arith NatAssertion where
+    coe e := fun s => e.eval s
+  instance: Coe Prop Assertion where
+    coe P := fun _ => P
+
   @[reducible]
   def Assertion.implies (P Q: Assertion): Assertion := fun s => P s → Q s
   def Assertion.iff (P Q: Assertion): Assertion := fun s => implies P Q s ∧ implies Q P s
   def Assertion.and (P Q: Assertion): Assertion := fun s => P s ∧ Q s
   def Assertion.or (P Q: Assertion): Assertion := fun s => P s ∨ Q s
   def Assertion.not (P: Assertion): Assertion := fun s => ¬ P s
-  def Assertion.eq (P Q: Assertion): Assertion := fun s => P s = Q s
-  def Assertion.neq (P Q: Assertion): Assertion := fun s => P s ≠ Q s
-  def Assertion.lt (P Q: Assertion): Assertion := fun s => P s < Q s
-  def Assertion.le (P Q: Assertion): Assertion := fun s => P s ≤ Q s
-  def Assertion.gt (P Q: Assertion): Assertion := fun s => P s > Q s
-  def Assertion.ge (P Q: Assertion): Assertion := fun s => P s ≥ Q s
-  -- def Assertion.add (P Q: Assertion): Assertion := fun s => P s + Q s
+  def Assertion.eq (P Q: NatAssertion): Assertion := fun s => P s = Q s
+  def Assertion.neq (P Q: NatAssertion): Assertion := fun s => P s ≠ Q s
+  def Assertion.lt (P Q: NatAssertion): Assertion := fun s => P s < Q s
+  def Assertion.le (P Q: NatAssertion): Assertion := fun s => P s ≤ Q s
+  def Assertion.gt (P Q: NatAssertion): Assertion := fun s => P s > Q s
+  def Assertion.ge (P Q: NatAssertion): Assertion := fun s => P s ≥ Q s
+  def Assertion.add (P Q: NatAssertion): NatAssertion := fun s => P s + Q s
+  def Assertion.sub (P Q: NatAssertion): NatAssertion := fun s => P s - Q s
+  def Assertion.mul (P Q: NatAssertion): NatAssertion := fun s => P s * Q s
+
+  def ap (f: Nat → α) (e: NatAssertion) := fun s => f (e s)
+  def ap₂ (f: Nat → Nat → a) (e₁ e₂: NatAssertion) := fun s => f (e₁ s) (e₂ s)
+
+  infix:65 "→" => Assertion.implies
+  infix:65 "↔" => Assertion.iff
+  infixr:35 "∧" => Assertion.and
+  infixr:30 "∨" => Assertion.or
+  notation:max "¬" P:40 => Assertion.not P
+  infix:50 "===" => Assertion.eq
+  infix:65 "≠" => Assertion.neq
+  infix:50 "<" => Assertion.lt
+  infix:50 "≤" => Assertion.le
+  infix:50 ">" => Assertion.gt
+  infix:50 "≥" => Assertion.ge
+
+  instance: Add NatAssertion where
+    add P Q := Assertion.add P Q
+  instance: Sub NatAssertion where
+    sub P Q := Assertion.sub P Q
+  instance: Mul NatAssertion where
+    mul P Q := Assertion.mul P Q
+
+  section
+    private def ex₁: Assertion := "X" === 3
+    private def ex₂: Assertion := True
+    private def ex₃: Assertion := False
+
+    private def ex₄: Assertion := "X" ≤ "Y"
+    private def ex₅: Assertion := ("X" === 3) ∨ (("X": NatAssertion) < "Y")
+    private def ex₆: Assertion := "X" === (ap₂ max "X" "Y")
+    private def ex₇: Assertion := ("Z" * "Z" ≤ "X") ∨ ¬((ap Nat.succ "Z") * (ap Nat.succ "Z") ≤ "X")
+  end
 
   /-
   ## Hoare Triples, Informally
@@ -51,10 +99,13 @@ namespace SoftwareFoundations.ProgrammingLanguageFoundations.Hoare
   def HoareTriple (P: Assertion) (c: Command) (Q: Assertion): Prop :=
     ∀ s₁ s₂: State, P s₁ → CommandEval c s₁ s₂ → Q s₂
 
-  theorem HoareTriple.post_true {P Q: Assertion} {c: Command}: (h: (s: State) → Q s) → HoareTriple P c Q
-    | h, s₁, s₂, hp, c => sorry
+  notation " ⦃ " P " , " c " , " Q " ⦄ " => HoareTriple P c Q
 
-  theorem HoareTriple.pre_false {P Q: Assertion} {c: Command}: (h: (s: State) → ¬P s) → HoareTriple P c Q
+  theorem HoareTriple.post_true {P Q: Assertion} {c: Command}: (h: (s: State) → Q s) → ⦃P, c, Q⦄
+    | h, s₁, s₂, hp, c =>
+      sorry
+
+  theorem HoareTriple.pre_false {P Q: Assertion} {c: Command}: (h: (s: State) → ¬P s) → ⦃P, c, Q⦄
     | h, s₁, s₂, hp, c => sorry
 
   /-
@@ -65,14 +116,14 @@ namespace SoftwareFoundations.ProgrammingLanguageFoundations.Hoare
   ### Skip
   -/
 
-  def HoareTriple.skip {P: Assertion}: HoareTriple P .skip P
+  def HoareTriple.skip {P: Assertion}: ⦃P, .skip, P⦄
     | _, _, hp, .skip _ => hp
 
   /-
   ### Sequencing
   -/
 
-  def HoareTriple.seq {P Q R: Assertion} {c₁ c₂: Command} (h₁: HoareTriple Q c₂ R) (h₂: HoareTriple P c₁ Q): HoareTriple P (.seq c₁ c₂) R
+  def HoareTriple.seq {P Q R: Assertion} {c₁ c₂: Command} (h₁: ⦃Q, c₂, R⦄) (h₂: ⦃P, c₁, Q⦄): ⦃P, (.seq c₁ c₂), R⦄
     | _, _, hp, .seq _ _ _ h₃ h₄ =>
       have hq := h₂ _ _ hp h₃
       h₁ _ _ hq h₄
@@ -85,16 +136,64 @@ namespace SoftwareFoundations.ProgrammingLanguageFoundations.Hoare
   def Assertion.subst (id: String) (e: Arith) (P: Assertion): Assertion
     | s => P (s.update id (e.eval s))
 
-  def HoareTriple.assign {Q: Assertion} {id: String} {e: Arith}: HoareTriple (Q.subst id e) (.assign id e) Q
-    | _,_, hqs, .assign _ h =>
-      -- TODO: Remove Tactic Block
-      by
-        unfold Assertion.subst at hqs
-        simp at hqs
-        rw [h] at hqs
-        exact hqs
+  notation P "[" id "↦" e "]" => Assertion.subst id e P
 
-  -- TODO: Complete assertions and implement example(s)
+  def HoareTriple.assign {Q: Assertion} {id: String} {e: Arith}: ⦃Q [id ↦ e], (.assign id e), Q⦄
+    | _,_, hqs, .assign _ h =>
+      have h :=
+        calc Assertion.subst id e Q _
+          _ = Q (LogicalFoundations.Maps.TotalMap.update _ id (Arith.eval _ e)) := rfl
+          _ = Q (LogicalFoundations.Maps.TotalMap.update _ id _)                := congrArg Q (congrArg (LogicalFoundations.Maps.TotalMap.update _ id) h)
+      -- TODO: Remove Tactic Block
+      by rw [h] at hqs; exact hqs
+
+  namespace Term
+    example: ⦃(Assertion.lt "X" 5) ["X" ↦ "X" + 1], .assign "X" ("X" + 1), Assertion.lt "X" 5⦄ :=
+      HoareTriple.assign
+
+    example: ∃ P, ⦃P, .assign "X" (2 * "X"), "X" ≤ 10⦄ :=
+      ⟨"X" ≤ 5, sorry⟩
+
+    example: ∃ P, ⦃P, .assign "X" 3, ("X" ≤ 0 ∧ "X" ≤ 5)⦄ :=
+      ⟨True, sorry⟩
+
+    example: ∃ E: Arith, ¬ ⦃True, .assign "X" e, "X" === e⦄ := sorry
+    example (n: Nat) (e: Arith) (P: Assertion): ⦃fun s => P s ∧ s "X" = n, .assign "X" e, fun s => P (s.update "X" n) ∧ s "X" = e.eval (s.update "X" n)⦄ := sorry
+    example (e: Arith) (P: Assertion): ⦃fun s => P s, .assign "X" e, fun s => ∃ n: Nat, P (s.update "X" n) ∧ s "X" = e.eval (s.update "X" n)⦄ := sorry
+  end Term
+
+  namespace Tactic
+    example: ⦃(Assertion.lt "X" 5) ["X" ↦ "X" + 1], .assign "X" ("X" + 1), Assertion.lt "X" 5⦄ := by
+      apply HoareTriple.assign
+
+    example: ∃ P, ⦃P, .assign "X" (2 * "X"), "X" ≤ 10⦄ := by
+      exists "X" ≤ 5
+      sorry
+
+    example: ∃ P, ⦃P, .assign "X" 3, ("X" ≤ 0 ∧ "X" ≤ 5)⦄ := by
+      exists True
+      sorry
+
+    example: ∃ E: Arith, ¬ ⦃True, .assign "X" e, "X" === e⦄ := by
+      sorry
+
+    example (n: Nat) (e: Arith) (P: Assertion): ⦃fun s => P s ∧ s "X" = n, .assign "X" e, fun s => P (s.update "X" n) ∧ s "X" = e.eval (s.update "X" n)⦄ := by
+      sorry
+
+    example (e: Arith) (P: Assertion): ⦃fun s => P s, .assign "X" e, fun s => ∃ n: Nat, P (s.update "X" n) ∧ s "X" = e.eval (s.update "X" n)⦄ := by
+      sorry
+  end Tactic
+
+  namespace Blended
+    example: ⦃(Assertion.lt "X" 5) ["X" ↦ "X" + 1], .assign "X" ("X" + 1), Assertion.lt "X" 5⦄ :=
+      HoareTriple.assign
+
+    example: ∃ P, ⦃P, .assign "X" (2 * "X"), "X" ≤ 10⦄ := sorry
+    example: ∃ P, ⦃P, .assign "X" 3, ("X" ≤ 0 ∧ "X" ≤ 5)⦄ := sorry
+    example: ∃ E: Arith, ¬ ⦃True, .assign "X" e, "X" === e⦄ := sorry
+    example (n: Nat) (e: Arith) (P: Assertion): ⦃fun s => P s ∧ s "X" = n, .assign "X" e, fun s => P (s.update "X" n) ∧ s "X" = e.eval (s.update "X" n)⦄ := sorry
+    example (e: Arith) (P: Assertion): ⦃fun s => P s, .assign "X" e, fun s => ∃ n: Nat, P (s.update "X" n) ∧ s "X" = e.eval (s.update "X" n)⦄ := sorry
+  end Blended
 
   /-
   ### Consequence
